WIP really big rewrite/simplification

Cook_Levin_IMP/IMP-_To_SAS+/IMP-_To_IMP--/Primitives.thy
@@ -12,6 +12,7 @@ theory Primitives
     SAS_Plus_Plus_To_SAS_Plus
     IMP_Minus_Minus_To_SAS_Plus_Plus_State_Translations
     "Poly_Reductions_Lib.Encode_Nat"
+    "HOL-Library.List_Lexorder"
 begin
 
 
@@ -36,15 +37,11 @@ declare enc_HOL_bool.simps[simp del]
 declare dec_HOL_bool.simps[simp del]
 
 datatype_nat_wellbehaved bool
-  by(simp add: dec_HOL_bool.simps enc_HOL_bool.simps split:bool.split)
+  by(intro ext, simp add: dec_HOL_bool.simps enc_HOL_bool.simps split:bool.split)
 
 thm enc_HOL_bool.simps
 thm dec_HOL_bool.simps
 thm HOL_bool_wellbehaved
-
-lemma inj_enc_HOL_bool: "inj enc_HOL_bool"
-  apply (rule inj_on_inverseI[of _ dec_HOL_bool])
-  using HOL_bool_wellbehaved by simp
 
 
 datatype_nat_encode char
@@ -55,31 +52,19 @@ declare enc_String_char.simps[simp del]
 declare dec_String_char.simps[simp del]
 
 datatype_nat_wellbehaved char
+  apply(intro ext)
   apply(simp add: enc_String_char.simps dec_String_char.simps)
-  apply(rule allI)
   subgoal
-    using HOL_bool_wellbehaved by (induction rule: char.induct) (simp)
+    using HOL_bool_wellbehaved by (induction rule: char.induct) (simp add: pointfree_idE)
   done
 
 thm enc_String_char.simps
 thm dec_String_char.simps
 thm String_char_wellbehaved
 
-lemma inj_enc_String_char: "inj enc_String_char"
-  apply (rule inj_on_inverseI[of _ dec_String_char])
-  using String_char_wellbehaved by simp
 
-lemma inj_enc_Nat_nat: "inj enc_Nat_nat"
-  apply (rule inj_on_inverseI[of _ dec_Nat_nat])
-  using Nat_nat_wellbehaved by simp
 
-lemma inj_enc_List_list:
-  assumes "inj enc_'a"
-    and "wellbehaved enc_'a dec_'a"
-  shows "inj (enc_List_list enc_'a)"
-  apply(rule inj_on_inverseI)
-  using assms(1) List_list_wellbehaved[OF assms(2)] by fastforce
-
+value "dec_String_char bot"
 
 (*
 definition encode_char :: "char \<Rightarrow> nat" where
@@ -109,98 +94,124 @@ lemma snd_helper_eq: "snd_helper = snd" by fastforce
 
 function_nat_rewrite fst_helper
 function_nat_rewrite_correctness fst_helper
-by (natfn_correctness \<open>induct arg\<^sub>1 rule: fst_helper.induct\<close>
-      assms: assms
-      simps_nat: fst_helper_nat.simps
-      enc_simps: enc_Product_Type_prod.simps
-      args_wellbehaved: Product_Type_prod_wellbehaved[OF assms(1)])
+  apply(induction arg\<^sub>1 rule: fst_helper.induct)
+  apply(all \<open>subst fst_helper_nat.simps\<close>)
+  subgoal for a b
+    apply(subst enc_Product_Type_prod.simps)
+    by(simp add: assms pointfree_idE enc_Product_Type_prod.simps)
+  done
 
 function_nat_rewrite snd_helper
 function_nat_rewrite_correctness snd_helper
-by (natfn_correctness \<open>induct arg\<^sub>1 rule: snd_helper.induct\<close>
+  by(natfn_correctness \<open>induct arg\<^sub>1 rule: snd_helper.induct\<close>
       assms: assms
       simps_nat: snd_helper_nat.simps
       enc_simps: enc_Product_Type_prod.simps
-      args_wellbehaved: Product_Type_prod_wellbehaved[OF assms(1)])
+      args_wellbehaved: assms[THEN pointfree_idE])
+(*
+  apply(induction arg\<^sub>1 rule: snd_helper.induct)
+  apply(all \<open>subst snd_helper_nat.simps\<close>)
+  subgoal for a b
+    apply(subst enc_Product_Type_prod.simps)
+    by(simp add: assms pointfree_idE enc_Product_Type_prod.simps)
+  done
+*)
 
 definition "fst_nat \<equiv> fst_helper_nat"
 definition "snd_nat \<equiv> snd_helper_nat"
 
 lemma fst_nat_equiv:
   assumes
-    "wellbehaved (enc_a::'a \<Rightarrow> nat) (dec_a::nat \<Rightarrow> 'a)" and
-    "wellbehaved (enc_b::'b \<Rightarrow> nat) (dec_b::nat \<Rightarrow> 'b)"
+    "dec_a \<circ> enc_a = id" and
+    "dec_b \<circ> enc_b = id"
   shows
   "dec_a (fst_nat (enc_Product_Type_prod enc_a enc_b p)) = fst p"
-  using fst_helper_nat_equiv[OF assms(1) assms(2), of p]
+  using fst_helper_nat_equiv[OF assms]
   by (subst fst_nat_def, subst fst_helper_eq[symmetric]) assumption
 
 lemma snd_nat_equiv:
   assumes
-    "wellbehaved (enc_a::'a \<Rightarrow> nat) (dec_a::nat \<Rightarrow> 'a)" and
-    "wellbehaved (enc_b::'b \<Rightarrow> nat) (dec_b::nat \<Rightarrow> 'b)"
+    "dec_a \<circ> enc_a = id" and
+    "dec_b \<circ> enc_b = id"
   shows
   "dec_b (snd_nat (enc_Product_Type_prod enc_a enc_b p)) = snd p"
-  using snd_helper_nat_equiv[OF assms(2) assms(1), of p]
+  using snd_helper_nat_equiv[OF assms(2) assms(1)]
   by (subst snd_nat_def, subst snd_helper_eq[symmetric]) assumption
-
-
-lemma sub_fst: "fst_nat (prod_encode p) = fst p"
-  apply (simp add: fst_nat_def)
-  oops
-
-lemma sub_snd: "snd_nat (prod_encode p) = snd p"
-  apply (simp add: snd_nat_def)
-  oops
-
-lemma "snd_nat xs \<le> xs"
-  (* apply (simp add: snd_nat_def) 
-    (metis le_prod_encode_2 prod.collapse prod_decode_inverse) *)
-  oops
 
 lemma eq: "prod_encode (n,m) = (m+n) * (m+n+1) div 2 + n"
   by (simp add: add.commute prod_encode_def triangle_def)
 
-definition hd_nat :: "nat \<Rightarrow> nat" where
-  "hd_nat xs = fst_nat (xs-1)"
 
-definition tl_nat :: "nat \<Rightarrow> nat" where
-  "tl_nat xs = snd_nat (xs-1)"
+fun head :: "'a list \<Rightarrow> 'a" where
+  "head (x # xs) = x"
+| "head [] = undefined"
 
-fun head :: "nat list \<Rightarrow> nat" where 
-  "head [] = 0"|
-  "head (x#xs) = x"
+fun head_bot :: "('a::order_bot) list \<Rightarrow> 'a" where
+  "head_bot (x # xs) = x"
+| "head_bot [] = bot"
 
-fun tail :: "nat list \<Rightarrow> nat list" where
-  "tail [] = []"|
-  "tail (x#xs) = xs"
+thm hd_def
 
-function_nat_rewrite head
-function_nat_rewrite_correctness head
-  using fst_prod_decode_lte fst_prod_decode_less
-  by (induction arg\<^sub>1 rule: head.induct)
-   (fastforce simp add: enc_List_list.simps prod_encode_def head_nat.simps,
-     simp add: enc_List_list.simps enc_Nat_nat.simps head_nat.simps)
+ML \<open>
+val T = @{typ "nat"};
+Term.is_Type T;
+Term.is_TFree T;
+Term.is_TVar T;
 
-fun ahead :: "'a list \<Rightarrow> 'a" where 
-  "ahead [] = undefined"|
-  "ahead (x#xs) = x"
+Ctr_Sugar.ctr_sugar_of @{context} "'a"
+\<close>
 
-ML \<open>Term.body_type\<close>
+term "bot::nat"
 
-function_nat_rewrite ahead
+ML \<open>
+@{term bot_nat}
+\<close>
+
+function_nat_rewrite head_bot
+thm head_bot_nat.simps
+function_nat_rewrite_correctness head_bot
+  apply(induction arg\<^sub>1 rule: head_bot.induct)
+   apply(all \<open>subst head_bot_nat.simps\<close>)
+  subgoal
+    using assms
+    by(simp add: pointfree_idE enc_Nat_nat.simps enc_List_list.simps)
+  subgoal
+    apply(simp add: enc_List_list.simps)
+    sorry
+  done
+
+fun tail :: "'a list \<Rightarrow> 'a list" where
+  "tail (x # xs) = xs"
+| "tail [] = []"
+
 
 function_nat_rewrite tail
 thm tail_nat.simps
 
-function_nat_rewrite_correctness tail
-  apply (induction arg\<^sub>1 rule: head.induct)
-   apply (all \<open>subst tail_nat.simps\<close>)
-  using List_list_wellbehaved[of enc_Nat_nat dec_Nat_nat, OF Nat_nat_wellbehaved]
-  by (simp add: enc_List_list.simps)+
 
-lemma "x = [] \<longleftrightarrow> enc_List_list enc_Nat_nat xs = 0"
-  using enc_List_list_inj
+function_nat_rewrite_correctness tail
+  by(natfn_correctness \<open>induct arg\<^sub>1 rule: tail.induct\<close>
+      assms: assms
+      simps_nat: tail_nat.simps
+      enc_simps: enc_List_list.simps
+      args_wellbehaved: List_list_wellbehaved[OF assms, THEN pointfree_idE])
+
+thm Encode_Nat.List_list_wellbehaved[of inj_on_imageI]
+thm inj_on_imageI[of ] Encode_Nat.List_list_wellbehaved
+thm inj_on_inverseI[of _ dec_List_list] List_list_wellbehaved
+thm
+lemma inj_enc_List_list:
+  assumes "inj enc_'a"
+    and "dec_'a \<circ> enc_'a = id"
+  shows "inj (enc_List_list enc_'a)"
+  apply(rule inj_on_inverseI)
+  using assms(1) List_list_wellbehaved[OF assms(2)]
+
+thm inj_on_inverseI[OF List_list_wellbehaved]
+
+
+lemma "x = [] \<longleftrightarrow> enc_List_list enc xs = 0"
+  apply(simp add: enc_List_list.simps)
 
 lemma "xs = [] \<longleftrightarrow> list_encode xs = 0"
   using list_encode_eq by force
@@ -216,12 +227,12 @@ lemma sub_tl :"tl_nat (list_encode xs) = list_encode (tail xs) "
       simp add: tl_nat_def sub_snd)
 
 lemma sub_head:" xs  \<noteq> [] \<Longrightarrow>head xs = hd xs"
-  apply (cases xs) 
+  apply (cases xs)
    apply (auto simp add: hd_nat_def)
   done
 
 lemma sub_tail :" xs \<noteq> [] \<Longrightarrow> tail xs = tl xs"
-  apply (cases xs) 
+  apply (cases xs)
    apply (auto simp add: tl_nat_def)
   done
 
@@ -231,18 +242,18 @@ lemma sub_tail :" xs \<noteq> [] \<Longrightarrow> tail xs = tl xs"
 lemma [simp]: " tl_nat (Suc v) < Suc v"
   apply (auto simp add:tl_nat_def snd_nat_def)
   by (metis le_imp_less_Suc le_prod_encode_2 prod.exhaust_sel prod_decode_inverse)
-  
+
 
 lemma [simp]:  "0 < xs \<Longrightarrow> list_encode (tail (list_decode xs)) < xs"
-  by (metis (no_types, lifting) Suc_diff_1 Suc_le_eq Suc_le_mono case_prod_beta tail.simps(2) 
- le_prod_encode_2 
+  by (metis (no_types, lifting) Suc_diff_1 Suc_le_eq Suc_le_mono case_prod_beta tail.simps(2)
+ le_prod_encode_2
 list_decode.simps(2) list_decode_inverse prod.exhaust_sel prod_decode_inverse)
-  
+
 lemma [simp]: "list_encode (tail (case prod_decode v of (x, y) \<Rightarrow> x # list_decode y)) < Suc v"
   by (metis case_prod_beta tail.simps(2) le_imp_less_Suc le_prod_encode_2
  list_decode_inverse prod.exhaust_sel prod_decode_inverse)
 
-fun length_nat :: "nat \<Rightarrow> nat" where 
+fun length_nat :: "nat \<Rightarrow> nat" where
 "length_nat 0 = 0"|
 "length_nat n = Suc (length_nat (tl_nat n))"
 
@@ -252,13 +263,13 @@ lemma non_empty_positive : "list_encode (a #xs) > 0" by simp
 lemma sub_length : "length_nat (list_encode xs) = length xs"
   apply (induct xs)
    apply (auto)
-  using tl_nat_def  by (simp add: snd_nat_def) 
-  
-  
-    
-  
+  using tl_nat_def  by (simp add: snd_nat_def)
 
-definition cons :: "nat \<Rightarrow> nat \<Rightarrow> nat" where 
+
+
+
+
+definition cons :: "nat \<Rightarrow> nat \<Rightarrow> nat" where
 "cons h t = Suc (prod_encode (h,t))"
 
 bundle cons_syntax
@@ -280,8 +291,8 @@ lemma [simp]: "0 < xs \<Longrightarrow> tl_nat xs < xs"
  add.left_neutral case_prod_beta comp_apply comp_def gr0_implies_Suc le_imp_less_Suc
  le_prod_encode_2 lessI plus_nat.simps(1) prod.simps(2) prod_decode_def prod_encode_def
  prod_encode_prod_decode_aux snd_nat_def split_conv tl_nat_def triangle_0)
-  
-fun takeWhile_nat :: "(nat \<Rightarrow> bool) \<Rightarrow> nat \<Rightarrow> nat" where 
+
+fun takeWhile_nat :: "(nat \<Rightarrow> bool) \<Rightarrow> nat \<Rightarrow> nat" where
 "takeWhile_nat P xs = (let h = hd_nat xs; t = tl_nat xs in (if xs = 0 then 0 else (if P h
             then cons h (takeWhile_nat P t) else 0)))"
 
@@ -291,20 +302,20 @@ lemma sub_takeWhile:"takeWhile_nat P (list_encode xs) = list_encode (takeWhile P
   by (smt cons_def head.simps(2) list.distinct(1) list_decode.simps(1) list_decode_inverse
  list_encode.simps(2) list_encode_eq sub_hd sub_tl tail.simps(2) takeWhile.simps(2)
  takeWhile_nat.simps)
- 
-  
-  
-  
-fun dropWhile_nat :: "(nat \<Rightarrow> bool) \<Rightarrow> nat \<Rightarrow> nat" where 
+
+
+
+
+fun dropWhile_nat :: "(nat \<Rightarrow> bool) \<Rightarrow> nat \<Rightarrow> nat" where
 "dropWhile_nat P xs = (let h = hd_nat xs; t = tl_nat xs in (if xs = 0 then 0 else (if P h
             then dropWhile_nat P t else xs)))  "
 
 lemma sub_dropWhile: "dropWhile_nat P (list_encode xs) = list_encode (dropWhile P xs)"
-  apply (induct xs) 
+  apply (induct xs)
    apply simp
-  by (metis dropWhile.simps(2) dropWhile_nat.elims head.simps(2) 
+  by (metis dropWhile.simps(2) dropWhile_nat.elims head.simps(2)
 list_decode_inverse nat_less_le non_empty_positive sub_hd sub_tl tail.simps(2))
-  
+
 
 datatype_nat_encode option
 declare enc_Option_option.simps[simp del]
@@ -339,11 +350,11 @@ lemma option_wellbehaved[simp]: "option_decode_auto (option_encode_auto xs) = xs
   apply(rule foo)
   using Option_option_wellbehaved Nat_nat_wellbehaved by fastforce
 
-fun option_decode :: "nat \<Rightarrow> nat option" where 
+fun option_decode :: "nat \<Rightarrow> nat option" where
 "option_decode 0 = None"|
 "option_decode (Suc x) = Some x"
 
-fun option_encode :: "nat option \<Rightarrow> nat" where 
+fun option_encode :: "nat option \<Rightarrow> nat" where
 "option_encode None = 0"|
 "option_encode (Some x) = Suc x"
 
@@ -352,15 +363,15 @@ lemma [simp]: "option_encode (option_decode xs) = xs"
 
 lemma [simp]: "option_decode (option_encode xs) = xs"
   by (metis option_decode.simps(1) option_decode.simps(2) option_encode.elims)
-  
-definition some_nat :: "nat \<Rightarrow> nat" where 
+
+definition some_nat :: "nat \<Rightarrow> nat" where
 "some_nat = Suc"
 lemma sub_some [simp]: "some_nat x = option_encode (Some x)"
   by (simp add: some_nat_def)
 
 
 
-   
+
 
 definition vname_encode_auto :: "string \<Rightarrow> nat" where
   "vname_encode_auto n = enc_List_list enc_String_char n"
@@ -368,29 +379,29 @@ definition vname_encode_auto :: "string \<Rightarrow> nat" where
 definition vname_decode_auto :: "nat \<Rightarrow> string" where
   "vname_decode_auto n = dec_List_list dec_String_char n"
 
-definition vname_encode :: "string \<Rightarrow> nat" where 
+definition vname_encode :: "string \<Rightarrow> nat" where
 "vname_encode v = list_encode (map encode_char v)"
 
-definition vname_decode :: "nat \<Rightarrow> string" where 
+definition vname_decode :: "nat \<Rightarrow> string" where
 "vname_decode v = map decode_char (list_decode v)"
 
 lemma vname_id: "vname_decode (vname_encode xs) = xs"
   by (auto simp add: vname_encode_def vname_decode_def idcharorg)
 
-lemma vname_inj: "inj vname_encode" 
+lemma vname_inj: "inj vname_encode"
   apply (auto simp add:inj_def)
   by (metis vname_id)
-   
-definition vname_list_encode :: "string list \<Rightarrow> nat" where 
+
+definition vname_list_encode :: "string list \<Rightarrow> nat" where
 "vname_list_encode l = list_encode (map vname_encode l)"
 
-definition vname_list_decode :: "nat \<Rightarrow> string list" where 
+definition vname_list_decode :: "nat \<Rightarrow> string list" where
 "vname_list_decode n = map vname_decode (list_decode n)"
 
 lemma vname_list_id:"vname_list_decode (vname_list_encode x) = x"
   by (auto simp add: vname_list_encode_def vname_list_decode_def map_idI vname_id)
 
-fun append_nat :: "nat \<Rightarrow> nat \<Rightarrow> nat" where 
+fun append_nat :: "nat \<Rightarrow> nat \<Rightarrow> nat" where
 "append_nat 0 ys = ys"|
 "append_nat xs ys = cons (hd_nat xs) (append_nat (tl_nat xs) ys)"
 
@@ -398,16 +409,16 @@ lemma sub_append: "append_nat (list_encode xs) (list_encode ys) = list_encode (x
   apply(induct xs)
    apply (auto simp only: append.simps sub_cons sub_hd sub_tl)
    apply auto
-  by (metis Suc_eq_plus1 add.commute add_diff_cancel_left' comp_def cons_def 
-head.simps(2) prod.sel(2) prod_encode_inverse snd_nat_def 
+  by (metis Suc_eq_plus1 add.commute add_diff_cancel_left' comp_def cons_def
+head.simps(2) prod.sel(2) prod_encode_inverse snd_nat_def
 sub_cons sub_hd tl_nat_def)
 
 
-fun append_acc :: "nat \<Rightarrow> nat \<Rightarrow> nat" where 
+fun append_acc :: "nat \<Rightarrow> nat \<Rightarrow> nat" where
 "append_acc acc 0 = acc"|
 "append_acc acc xs = append_acc ((hd_nat xs)## acc) (tl_nat xs)"
 
-fun reverse_nat_acc :: "nat \<Rightarrow>nat \<Rightarrow> nat" where 
+fun reverse_nat_acc :: "nat \<Rightarrow>nat \<Rightarrow> nat" where
 "reverse_nat_acc acc n = (if n = 0 then acc else reverse_nat_acc ((hd_nat n) ## acc) (tl_nat n) )"
 
 lemma sub_reverse_nat_acc:"reverse_nat_acc (list_encode acc) (list_encode n) = list_encode (rev n @ acc) "
@@ -418,44 +429,44 @@ lemma sub_reverse_nat_acc:"reverse_nat_acc (list_encode acc) (list_encode n) = l
   apply auto
   done
 
-definition reverse_nat :: "nat \<Rightarrow> nat" where 
+definition reverse_nat :: "nat \<Rightarrow> nat" where
 "reverse_nat n = reverse_nat_acc 0 n"
 
 lemma sub_reverse:"reverse_nat (list_encode n) = list_encode (rev n)"
   apply(auto simp only: reverse_nat_def )
-  using sub_reverse_nat_acc list_encode.simps(1) 
+  using sub_reverse_nat_acc list_encode.simps(1)
   by (metis append_Nil2)
 lemma reverse_nat_0:"(reverse_nat 0 =0)" by (auto simp add:reverse_nat_def)
 
 lemma append_rev_nat:"append_nat (reverse_nat (Suc v)) xs = append_nat (reverse_nat (tl_nat (Suc v))) ((hd_nat (Suc v)) ## xs)"
 proof-
-  obtain ys where xs_def: "Suc v = list_encode ys" 
+  obtain ys where xs_def: "Suc v = list_encode ys"
     by (metis list_decode_inverse)
   then moreover obtain a ys' where xs_def_cons : "ys = a#ys'"
     by (metis list_encode.elims nat.simps(3))
   moreover obtain xs_list where "xs = list_encode xs_list"  by (metis list_decode_inverse)
-  ultimately show ?thesis by (auto simp add: sub_reverse sub_tl sub_hd sub_cons 
+  ultimately show ?thesis by (auto simp add: sub_reverse sub_tl sub_hd sub_cons
           sub_append simp del: list_encode.simps)
 qed
 lemma append_cons_nat_0 : "append_nat xs (a ## ys) \<noteq> 0"
 proof-
-  obtain ys' where xs_def: "ys = list_encode ys'" 
+  obtain ys' where xs_def: "ys = list_encode ys'"
     by (metis list_decode_inverse)
   moreover obtain xs' where xs_def_cons : "xs = list_encode xs'"
    by (metis list_decode_inverse)
-  ultimately show ?thesis by (auto simp add: sub_reverse sub_tl sub_hd sub_cons 
+  ultimately show ?thesis by (auto simp add: sub_reverse sub_tl sub_hd sub_cons
           sub_append list_encode_eq simp flip: list_encode.simps)
 qed
 lemma cons_Nil:"xs ## ys \<noteq> 0"
 proof-
-  obtain ys' where xs_def: "ys = list_encode ys'" 
+  obtain ys' where xs_def: "ys = list_encode ys'"
     by (metis list_decode_inverse)
-  then show ?thesis by (auto simp add: sub_cons 
+  then show ?thesis by (auto simp add: sub_cons
           list_encode_eq simp flip: list_encode.simps)
 qed
 lemma tl_cons: "tl_nat (a##ys) = ys"
 proof-
-  obtain ys' where xs_def: "ys = list_encode ys'" 
+  obtain ys' where xs_def: "ys = list_encode ys'"
     by (metis list_decode_inverse)
   then show ?thesis by (auto simp add: sub_cons sub_tl
           list_encode_eq simp flip: list_encode.simps)
@@ -463,14 +474,14 @@ qed
 
 lemma hd_cons: "hd_nat (a##ys) = a"
 proof-
-  obtain ys' where xs_def: "ys = list_encode ys'" 
+  obtain ys' where xs_def: "ys = list_encode ys'"
     by (metis list_decode_inverse)
   then show ?thesis by (auto simp add: sub_cons sub_hd
           list_encode_eq simp flip: list_encode.simps)
 qed
 lemma rev_rev_nat: "reverse_nat (reverse_nat ys) = ys"
  proof-
-  obtain ys' where xs_def: "ys = list_encode ys'" 
+  obtain ys' where xs_def: "ys = list_encode ys'"
     by (metis list_decode_inverse)
   then show ?thesis by (auto simp add: sub_cons sub_reverse sub_hd
           list_encode_eq simp flip: list_encode.simps)
@@ -479,7 +490,7 @@ qed
 
 lemma append_nat_0: "append_nat ys 0 = ys"
 proof-
-  obtain ys' where xs_def: "ys = list_encode ys'" 
+  obtain ys' where xs_def: "ys = list_encode ys'"
     by (metis list_decode_inverse)
   then show ?thesis by (auto simp add: sub_append sub_hd
           list_encode_eq simp flip: list_encode.simps)
@@ -487,30 +498,30 @@ qed
 lemma cons0:"cons a 0 = list_encode [a]"
   by (metis list_encode.simps(1) sub_cons)
 
-lemma append_nat_Suc: 
+lemma append_nat_Suc:
 "append_nat xs (Suc v) = append_nat (append_nat xs ((hd_nat (Suc v))##0)) (tl_nat (Suc v))"
 proof -
   obtain xs' v' where "xs =list_encode xs'" "Suc v = list_encode v'"
     by (metis list_decode_inverse)
-  then moreover obtain a ys where "v' = a # ys" 
+  then moreover obtain a ys where "v' = a # ys"
     by (metis Zero_neq_Suc list_encode.elims)
-  ultimately show ?thesis apply(auto simp add:sub_append  sub_hd cons0 
+  ultimately show ?thesis apply(auto simp add:sub_append  sub_hd cons0
               sub_tl simp del:list_encode.simps) done
 qed
 
 lemma reverse_append_nat:
     "reverse_nat (append_nat xs ys) = append_nat (reverse_nat ys) (reverse_nat xs)"
-proof - 
+proof -
 obtain xs' ys' where "xs =list_encode xs'"  "ys = list_encode ys'"
   by (metis list_decode_inverse)
   thus ?thesis by(auto simp del:append_nat.simps list_encode.simps simp add: cons0 sub_cons
           sub_append sub_reverse)
 qed
 lemma reverse_singleton_nat:
-"reverse_nat (a ## 0) = a ## 0" by(auto simp add: cons0 sub_reverse simp del:list_encode.simps) 
-lemma append_singleton_nat : 
+"reverse_nat (a ## 0) = a ## 0" by(auto simp add: cons0 sub_reverse simp del:list_encode.simps)
+lemma append_singleton_nat :
 "append_nat (a##0) xs = a ## xs"
-proof - 
+proof -
   obtain xs' where "xs = list_encode xs'"
  by (metis list_decode_inverse)
   thus ?thesis by(auto simp del:append_nat.simps list_encode.simps simp add: cons0 sub_cons
@@ -520,33 +531,33 @@ qed
 lemma reverse_cons_nat:
 "reverse_nat (a ## xs) = append_nat (reverse_nat xs) (a##0) "
 proof -
-  obtain xs' where "xs= list_encode xs'" 
+  obtain xs' where "xs= list_encode xs'"
     by (metis list_decode_inverse)
-  thus ?thesis 
+  thus ?thesis
     apply (auto simp add:sub_append sub_reverse sub_cons cons0 simp del:
                   list_encode.simps) done
 qed
 
 lemma cons_is_reverse: "a ## reverse_nat xs = reverse_nat (append_nat xs (a##0))"
 proof -
-  obtain xs' where "xs= list_encode xs'" 
+  obtain xs' where "xs= list_encode xs'"
     by (metis list_decode_inverse)
-  thus ?thesis 
+  thus ?thesis
     apply (auto simp add:sub_append sub_reverse sub_cons cons0 simp del:
                   list_encode.simps) done
 qed
 
-lemma append_induct: " reverse_nat(append_nat xs ys) = 
+lemma append_induct: " reverse_nat(append_nat xs ys) =
 
 append_acc (reverse_nat xs) ys"
   apply(induct ys  arbitrary: xs rule:length_nat.induct)
    apply(simp add: append_nat_0)
-  apply (auto simp add: append_nat_Suc   reverse_append_nat reverse_singleton_nat 
+  apply (auto simp add: append_nat_Suc   reverse_append_nat reverse_singleton_nat
 append_singleton_nat simp flip: reverse_cons_nat)
   apply(auto simp only: cons_is_reverse)
   done
 
-definition append_tail :: "nat \<Rightarrow> nat \<Rightarrow> nat" where 
+definition append_tail :: "nat \<Rightarrow> nat \<Rightarrow> nat" where
 "append_tail xs ys = reverse_nat (append_acc (reverse_nat xs) ys)"
 
 lemma subtail_append:
@@ -556,7 +567,7 @@ lemma subtail_append:
   by (metis append_induct)
 
 
-fun elemof :: "nat \<Rightarrow> nat \<Rightarrow> nat" where 
+fun elemof :: "nat \<Rightarrow> nat \<Rightarrow> nat" where
 "elemof e l = (if l = 0 then 0 else if hd_nat l = e then 1 else elemof e (tl_nat l))"
 
 lemma sub_elem_of: "elemof e (list_encode l) \<noteq> 0 =  (e \<in> set l)"
@@ -564,8 +575,8 @@ lemma sub_elem_of: "elemof e (list_encode l) \<noteq> 0 =  (e \<in> set l)"
    apply (subst elemof.simps)
    apply(simp add: sub_hd sub_tl del:elemof.simps)
   apply (subst elemof.simps)
-  apply (auto simp only: sub_hd sub_tl sub_tail sub_head head.simps tl_def list.distinct(2) 
-split:if_splits 
+  apply (auto simp only: sub_hd sub_tl sub_tail sub_head head.simps tl_def list.distinct(2)
+split:if_splits
         del:elemof.simps)
            apply (auto)
   done
@@ -573,11 +584,11 @@ split:if_splits
 lemma sub_elem_of2: "(elemof e (list_encode l) = 0) =  (e \<notin> set l)"
   using sub_elem_of by blast
 
-fun remdups_nat :: "nat \<Rightarrow> nat" where 
+fun remdups_nat :: "nat \<Rightarrow> nat" where
 "remdups_nat n = (if n=0 then 0 else if elemof (hd_nat n) (tl_nat n) \<noteq> 0 then remdups_nat (tl_nat n)
                  else cons (hd_nat n) (remdups_nat (tl_nat n)))"
 
-fun remdups_acc :: "nat \<Rightarrow> nat => nat" where 
+fun remdups_acc :: "nat \<Rightarrow> nat => nat" where
 "remdups_acc acc n =(if n=0 then acc else if elemof (hd_nat n) (tl_nat n) \<noteq> 0 then remdups_acc acc (tl_nat n)
                  else remdups_acc (cons (hd_nat n) acc) (tl_nat n))"
 
@@ -587,10 +598,10 @@ lemma sub_remdups: "remdups_nat (list_encode xs) = list_encode (remdups xs)"
    apply (auto simp only: sub_hd sub_tl tail.simps head.simps sub_tail sub_head remdups.simps sub_elem_of
         sub_cons)
    apply auto[1]
-  by (smt less_numeral_extra(3) non_empty_positive remdups_nat.elims sub_cons 
+  by (smt less_numeral_extra(3) non_empty_positive remdups_nat.elims sub_cons
 sub_elem_of sub_hd sub_tl)
 lemma non_empty_not_zero:"list_encode (a#xs) \<noteq> 0" using non_empty_positive by auto
-lemma remdups_induct : 
+lemma remdups_induct :
 " reverse_nat (append_nat (reverse_nat acc) (remdups_nat xs))
 = remdups_acc acc xs "
 proof -
@@ -605,7 +616,7 @@ simp del: list_encode.simps remdups_acc.simps append_nat.simps elemof.simps)
     done
 qed
 
-definition remdups_tail :: "nat \<Rightarrow> nat" where 
+definition remdups_tail :: "nat \<Rightarrow> nat" where
 "remdups_tail xs = reverse_nat (remdups_acc 0 xs)"
 
 lemma subtail_remdups:
@@ -615,9 +626,9 @@ lemma subtail_remdups:
   by (metis append_nat.simps(1) rev_rev_nat reverse_nat_0)
 
 lemma prod_sum_less:"0< x \<Longrightarrow>(x,y) = prod_decode p  \<Longrightarrow> x+y < p"
-  by (smt Nat.add_0_right Suc_leI add.left_commute add.left_neutral add.right_neutral 
+  by (smt Nat.add_0_right Suc_leI add.left_commute add.left_neutral add.right_neutral
 add_Suc_right add_mono_thms_linordered_semiring(1) canonically_ordered_monoid_add_class.lessE
- comm_monoid_add_class.add_0 le_imp_less_Suc le_prod_encode_2 not_le plus_nat.add_0 prod.simps(2) 
+ comm_monoid_add_class.add_0 le_imp_less_Suc le_prod_encode_2 not_le plus_nat.add_0 prod.simps(2)
 prod_decode_inverse prod_encode_def prod_encode_def split_conv)
 
 lemma prod_sum_less2:"(x,y) = prod_decode p  \<Longrightarrow> x+y \<le> p"
@@ -639,11 +650,11 @@ lemma prod_fst_less2:"(x,y) = prod_decode p  \<Longrightarrow> x \<le> p"
   by (metis le_prod_encode_1 prod_decode_inverse)
 
 
-fun atomExp_encode :: "atomExp \<Rightarrow> nat" where 
-"atomExp_encode (V var) = prod_encode (0, vname_encode var)" | 
+fun atomExp_encode :: "atomExp \<Rightarrow> nat" where
+"atomExp_encode (V var) = prod_encode (0, vname_encode var)" |
 "atomExp_encode (N n)   = prod_encode (1,n) "
 
-definition atomExp_decode :: "nat \<Rightarrow> atomExp" where 
+definition atomExp_decode :: "nat \<Rightarrow> atomExp" where
 "atomExp_decode n = (case prod_decode n of (0,v) \<Rightarrow> V (vname_decode v) | (Suc 0,n) \<Rightarrow> N n)"
 
 lemma atomExp_id:"atomExp_decode (atomExp_encode x) = x"
@@ -651,14 +662,14 @@ lemma atomExp_id:"atomExp_decode (atomExp_encode x) = x"
    apply (auto simp add: atomExp_decode_def vname_id)
   done
 
-fun aexp_encode :: "aexp \<Rightarrow> nat" where 
+fun aexp_encode :: "aexp \<Rightarrow> nat" where
 "aexp_encode (A a) = list_encode [0, atomExp_encode a]"|
 "aexp_encode (Plus a b) = list_encode [1,atomExp_encode a, atomExp_encode b]"|
 "aexp_encode (Sub a b) = list_encode  [2, atomExp_encode a, atomExp_encode b]"|
 "aexp_encode (Parity a) = list_encode [3, atomExp_encode a]"|
 "aexp_encode (RightShift a) = list_encode [4,atomExp_encode a]"
 
-fun aexp_decode :: "nat \<Rightarrow> aexp" where 
+fun aexp_decode :: "nat \<Rightarrow> aexp" where
 "aexp_decode n = (case list_decode n of
                     [0,a] \<Rightarrow> A (atomExp_decode a)|
                     [Suc 0,a,b] \<Rightarrow> Plus (atomExp_decode a) (atomExp_decode b)|
@@ -677,41 +688,41 @@ lemma set_less_helper: "x \<in>set xs \<Longrightarrow> x < list_encode xs"
   using le_imp_less_Suc le_prod_encode_1 apply blast
   by (meson Suc_lessD le_imp_less_Suc le_prod_encode_2 less_trans_Suc)
 
-lemma set_less [simp]: "x \<in>set (list_decode n) \<Longrightarrow> x < n"   
+lemma set_less [simp]: "x \<in>set (list_decode n) \<Longrightarrow> x < n"
 proof -
   assume assms:"x \<in>set (list_decode n) "
   obtain xs where "list_decode n = xs" by auto
-  then moreover have "n = list_encode xs" by auto 
+  then moreover have "n = list_encode xs" by auto
   thus ?thesis using assms by (auto simp add:set_less_helper)
 qed
 
-fun com_encode :: "IMP_Minus_com \<Rightarrow> nat" where 
+fun com_encode :: "IMP_Minus_com \<Rightarrow> nat" where
 "com_encode (Com.com.SKIP) = list_encode [0]"|
 "com_encode (Com.com.Assign vname aexp) = list_encode [1,vname_encode vname, aexp_encode aexp]"|
 "com_encode (Com.com.Seq c1 c2) = list_encode [2,com_encode c1,com_encode c2]"|
 "com_encode (Com.com.If v c1 c2) = list_encode [3, vname_encode v,com_encode c1,com_encode c2]"|
 "com_encode (Com.com.While v c) = list_encode [4,vname_encode v, com_encode c]"
 
-fun com_decode :: "nat \<Rightarrow> Com.com" where 
+fun com_decode :: "nat \<Rightarrow> Com.com" where
 "com_decode n = (case list_decode n of
                   [0] \<Rightarrow> Com.com.SKIP |
                   [Suc 0,v,a] \<Rightarrow> Com.com.Assign (vname_decode v) (aexp_decode a)|
                   [Suc (Suc 0),c1,c2] \<Rightarrow> Com.com.Seq (com_decode c1) (com_decode c2) |
                   [Suc(Suc (Suc 0)),v,c1,c2] \<Rightarrow> Com.com.If (vname_decode v) (com_decode c1) (com_decode c2)|
                   [Suc (Suc (Suc (Suc 0))),v,c] \<Rightarrow> Com.com.While  (vname_decode v) (com_decode c)
-)" 
-  
-lemma com_id: "com_decode (com_encode x) = x" 
+)"
+
+lemma com_id: "com_decode (com_encode x) = x"
   apply (subst com_encode.simps com_decode.simps)
   apply (induct x)
   apply (auto simp add: vname_id aexp_id simp del:aexp_encode.simps aexp_decode.simps )
   done
 
-fun bit_encode :: "bit \<Rightarrow> nat" where 
+fun bit_encode :: "bit \<Rightarrow> nat" where
 "bit_encode Zero = 0"|
 "bit_encode One = 1"
 
-fun bit_decode :: "nat \<Rightarrow> bit" where 
+fun bit_decode :: "nat \<Rightarrow> bit" where
 "bit_decode 0 = Zero"|
 "bit_decode (Suc 0) = One"
 
@@ -719,34 +730,34 @@ lemma bit_id[simp]: "bit_decode (bit_encode x) = x"
   by (cases x) auto
 
 
-fun comm_encode :: "com \<Rightarrow> nat" where 
+fun comm_encode :: "com \<Rightarrow> nat" where
 "comm_encode SKIP = list_encode [0]"|
 "comm_encode (Assign vname b) = list_encode [1,vname_encode vname, bit_encode b]"|
 "comm_encode (Seq c1 c2) = list_encode [2,comm_encode c1,comm_encode c2]"|
 "comm_encode (If v c1 c2) = list_encode [3, vname_list_encode v,comm_encode c1,comm_encode c2]"|
 "comm_encode (While v c) = list_encode [4,vname_list_encode v, comm_encode c]"
 
-fun comm_decode :: "nat \<Rightarrow> com" where 
+fun comm_decode :: "nat \<Rightarrow> com" where
 "comm_decode n = (case list_decode n of
                   [0] \<Rightarrow> SKIP |
                   [Suc 0,v,a] \<Rightarrow> Assign (vname_decode v) (bit_decode a)|
                   [Suc (Suc 0),c1,c2] \<Rightarrow> Seq (comm_decode c1) (comm_decode c2) |
                   [Suc(Suc (Suc 0)),v,c1,c2] \<Rightarrow> If (vname_list_decode v) (comm_decode c1) (comm_decode c2)|
                   [Suc (Suc (Suc (Suc 0))),v,c] \<Rightarrow> While (vname_list_decode v) (comm_decode c)
-)" 
+)"
 
-lemma comm_id: "comm_decode (comm_encode x) = x" 
+lemma comm_id: "comm_decode (comm_encode x) = x"
   apply (subst comm_encode.simps comm_decode.simps)
   apply (induct x)
   apply (auto simp add:vname_id vname_list_id)
   done
 
-fun nth :: "nat \<Rightarrow> nat list \<Rightarrow> nat" where 
+fun nth :: "nat \<Rightarrow> nat list \<Rightarrow> nat" where
 "nth n [] = 0"|
 "nth 0 (x#xs) = x"|
 "nth (Suc n) (x#xs) = nth n xs"
 
-fun nth_nat :: "nat \<Rightarrow> nat\<Rightarrow> nat" where 
+fun nth_nat :: "nat \<Rightarrow> nat\<Rightarrow> nat" where
 "nth_nat 0 x = hd_nat x "|
 "nth_nat (Suc n) x = nth_nat n (tl_nat x)"
 
@@ -772,15 +783,15 @@ lemma pos_tl_less[termination_simp]: "x > 0 \<Longrightarrow> tl_nat x < x"
 lemma nth_less[simp]: "nth_nat n x \<le> x"
   apply(induct n arbitrary:x)
    apply(auto simp add:hd_nat_def tl_nat_def snd_nat_def)
-   apply (metis comp_def diff_le_self fst_nat_def le_less_trans le_prod_encode_1 not_le 
+   apply (metis comp_def diff_le_self fst_nat_def le_less_trans le_prod_encode_1 not_le
 prod.exhaust_sel prod_decode_inverse)
   by (metis diff_le_self le_less_trans less_Suc_eq_le prod.exhaust_sel prod_snd_less2)
 
-   
+
 lemma [simp]: "x>0 \<Longrightarrow> nth_nat n x < x"
   apply (induct n arbitrary:x)
    apply (auto simp add:hd_nat_def fst_nat_def fst_def)
-   apply (metis Suc_pred case_prod_beta leI le_prod_encode_1 
+   apply (metis Suc_pred case_prod_beta leI le_prod_encode_1
 not_less_eq_eq prod.exhaust_sel prod_decode_inverse)
   subgoal for n x
     using pos_tl_less[of x] nth_less[of n "tl_nat x"]
@@ -788,7 +799,7 @@ not_less_eq_eq prod.exhaust_sel prod_decode_inverse)
   done
 
 
-fun map_nat :: "(nat\<Rightarrow> nat) \<Rightarrow> nat \<Rightarrow> nat" where 
+fun map_nat :: "(nat\<Rightarrow> nat) \<Rightarrow> nat \<Rightarrow> nat" where
 "map_nat f n= (if n =0 then 0 else cons (f (hd_nat n)) (map_nat f (tl_nat n)))"
 
 lemma sub_map:"map_nat f (list_encode xs) = list_encode (map f xs)"
@@ -804,7 +815,7 @@ fun num_to_list:: "num \<Rightarrow> nat list" where
 "num_to_list (num.Bit0 n) = 0#num_to_list n"|
 "num_to_list (num.Bit1 n) = 1#num_to_list n"
 
-fun list_to_num :: "nat list \<Rightarrow> num" where 
+fun list_to_num :: "nat list \<Rightarrow> num" where
 "list_to_num [] = num.One"|
 "list_to_num (0#xs) = num.Bit0 (list_to_num xs)"|
 "list_to_num (Suc 0#xs) = num.Bit1 (list_to_num xs)"
@@ -814,10 +825,10 @@ lemma list_to_num_id: "list_to_num (num_to_list n) = n"
     apply auto
   done
 
-definition num_encode :: "num \<Rightarrow> nat" where 
+definition num_encode :: "num \<Rightarrow> nat" where
 "num_encode x = list_encode (num_to_list x) "
 
-definition num_decode :: "nat \<Rightarrow> num" where 
+definition num_decode :: "nat \<Rightarrow> num" where
 "num_decode x = list_to_num (list_decode x)"
 
 lemma numid: "num_decode (num_encode x) = x"
@@ -835,10 +846,10 @@ lemma sub_tail_map : "tail (map f v) = map f (tl v)"
   done
 
 
-fun list_from_nat :: "nat \<Rightarrow> nat \<Rightarrow> nat" where 
+fun list_from_nat :: "nat \<Rightarrow> nat \<Rightarrow> nat" where
 "list_from_nat s n = (if n = 0 then 0 else cons s (list_from_nat (s+1) (n-1)))"
 
-fun list_from_acc :: "nat \<Rightarrow> nat \<Rightarrow> nat \<Rightarrow> nat" where 
+fun list_from_acc :: "nat \<Rightarrow> nat \<Rightarrow> nat \<Rightarrow> nat" where
 "list_from_acc acc s n = (if n = 0 then acc else list_from_acc (s ## acc) (s+1) (n-1) )  "
 
 lemma Suc_plus:"Suc(m+n) = Suc m + n "
@@ -858,7 +869,7 @@ lemma list_from_reverse:
 
 lemma list_from_induct:
 "reverse_nat (list_from_nat s (n+m)) =
-list_from_acc (reverse_nat (list_from_nat s n)) (s+n) m 
+list_from_acc (reverse_nat (list_from_nat s n)) (s+n) m
 "
   apply(induct m arbitrary: n)
    apply (simp)
@@ -871,13 +882,13 @@ list_from_acc (reverse_nat (list_from_nat s n)) (s+n) m
     done
   done
 
-definition list_from_tail :: "nat \<Rightarrow> nat \<Rightarrow> nat" where 
+definition list_from_tail :: "nat \<Rightarrow> nat \<Rightarrow> nat" where
 "list_from_tail s n = reverse_nat (list_from_acc 0 s n)"
 
-lemma subtail_list_from: 
+lemma subtail_list_from:
 "list_from_tail s n = list_from_nat s n"
   apply(auto simp only: list_from_tail_def)
-  using list_from_induct[of s 0 n] list_from_nat.simps reverse_nat_0 rev_rev_nat 
+  using list_from_induct[of s 0 n] list_from_nat.simps reverse_nat_0 rev_rev_nat
   by (metis add.left_neutral nat_arith.rule0)
 
 definition list_less_nat :: "nat \<Rightarrow> nat" where
@@ -886,11 +897,11 @@ definition list_less_nat :: "nat \<Rightarrow> nat" where
 definition list_less_tail :: "nat \<Rightarrow> nat" where
 "list_less_tail n = list_from_tail 0 n"
 
-lemma subtail_list_less : 
+lemma subtail_list_less :
 "list_less_tail n = list_less_nat n"
   apply(auto simp only: list_less_tail_def list_less_nat_def subtail_list_from)
   done
-  
+
 lemma sub_list_less : "list_less_nat n = list_encode ([0..<n])"
   apply (simp only: list_less_nat_def sub_list_from)
   apply auto
@@ -903,10 +914,10 @@ lemma comm_inj : "inj comm_encode"
   apply (induct c1 arbitrary: c2)
           apply (auto simp only: comm_encode.simps list_encode_eq comm_encode.elims)
   using comm_id apply (metis comm_encode.simps)
-  using comm_id apply (metis comm_encode.simps) 
-  using comm_id apply (metis comm_encode.simps) 
-  using comm_id apply (metis comm_encode.simps) 
-  done    
+  using comm_id apply (metis comm_encode.simps)
+  using comm_id apply (metis comm_encode.simps)
+  using comm_id apply (metis comm_encode.simps)
+  done
   done
 
 lemma remdups_map : "inj f \<Longrightarrow> remdups (map f xs) = map f (remdups xs)"
@@ -930,14 +941,14 @@ lemma sub_concat : "concat_nat (list_encode (map list_encode xs)) = list_encode 
 
 lemma conc_append: "concat xs @ a = concat(xs @ [a])" by auto
 find_theorems "rev _ @ rev _"
-lemma concat_induct: 
+lemma concat_induct:
 "reverse_nat (concat_nat (append_nat xs ys))
 = concat_acc (reverse_nat (concat_nat xs)) ys"
 proof -
   obtain xs' ys' where "xs =list_encode (map list_encode xs')" "ys = list_encode (map list_encode ys')"
     by (metis ex_map_conv list_decode_inverse)
-  thus ?thesis 
-    apply(auto simp add: sub_append sub_concat sub_reverse 
+  thus ?thesis
+    apply(auto simp add: sub_append sub_concat sub_reverse
        simp flip: map_append  simp del: list_encode.simps append_nat.simps concat_nat.simps concat_acc.simps)
     apply(induct ys' arbitrary:xs' xs ys)
      apply (simp)
@@ -946,11 +957,11 @@ proof -
      apply(simp)
     apply(auto simp add: sub_tl sub_hd  sub_append subtail_append  sub_reverse
            simp del: list_encode.simps append_nat.simps concat_nat.simps concat_acc.simps)
-    apply(auto simp only: conc_append simp flip: rev_append ) 
+    apply(auto simp only: conc_append simp flip: rev_append )
     done
 qed
 
-definition concat_tail:: "nat \<Rightarrow> nat" where 
+definition concat_tail:: "nat \<Rightarrow> nat" where
 "concat_tail ys = reverse_nat (concat_acc 0 ys)"
 
 lemma subtail_concat:
@@ -965,11 +976,11 @@ lemma vname_list_encode_as_comp:"vname_list_encode = list_encode o (map vname_en
 
 
 
-fun domain_element_encode ::"domain_element \<Rightarrow> nat" where 
+fun domain_element_encode ::"domain_element \<Rightarrow> nat" where
 "domain_element_encode (EV b) = prod_encode (0,bit_encode b)"|
 "domain_element_encode (PCV com) = prod_encode (1,comm_encode com)"
 
-fun domain_element_decode :: "nat \<Rightarrow> domain_element" where 
+fun domain_element_decode :: "nat \<Rightarrow> domain_element" where
 "domain_element_decode n = (case prod_decode n of
                             (0,b) \<Rightarrow> EV (bit_decode b)|
                             (Suc 0 , com) \<Rightarrow> PCV (comm_decode com)) "
@@ -982,11 +993,11 @@ lemma domain_element_id : "domain_element_decode (domain_element_encode x) = x"
    apply auto
   done
 
-fun variable_encode :: "variable \<Rightarrow> nat" where 
+fun variable_encode :: "variable \<Rightarrow> nat" where
 "variable_encode PC = 0"|
 "variable_encode (VN vn) = Suc (vname_encode vn)"
 
-fun variable_decode :: "nat \<Rightarrow> variable" where 
+fun variable_decode :: "nat \<Rightarrow> variable" where
 "variable_decode 0 = PC"|
 "variable_decode (Suc n) = VN (vname_decode n)"
 
@@ -995,7 +1006,7 @@ lemma variable_id : "variable_decode (variable_encode x) = x"
    apply (auto simp add: vname_id)
   done
 
-  
+
 lemma variable_inj : "inj variable_encode"
   apply (auto simp add:inj_def)
   subgoal for x y
@@ -1010,8 +1021,8 @@ lemma variable_inj : "inj variable_encode"
     done
   done
 
-      
-fun sas_assignment_encode:: "variable * domain_element \<Rightarrow> nat" where 
+
+fun sas_assignment_encode:: "variable * domain_element \<Rightarrow> nat" where
 "sas_assignment_encode (v,d) = prod_encode (variable_encode v, domain_element_encode d)"
 
 fun sas_assignment_decode:: "nat \<Rightarrow> (variable * domain_element) " where
@@ -1023,11 +1034,11 @@ lemma  sas_assignment_id: "sas_assignment_decode (sas_assignment_encode x) = x"
         prod_encode_inverse)
   done
 
-fun someOf :: "'a option \<Rightarrow> 'a" where 
+fun someOf :: "'a option \<Rightarrow> 'a" where
 "someOf (Some x) = x"
 
 
-definition map_to_list :: "('a,'b) map \<Rightarrow> ('a*'b) list" where 
+definition map_to_list :: "('a,'b) map \<Rightarrow> ('a*'b) list" where
 "map_to_list s \<equiv> (SOME l. map_of l = s)"
 
 lemma has_map:
@@ -1039,12 +1050,12 @@ proof -
   then show  "\<exists>l. map_of l = s " using assms
 proof (induct n arbitrary:s)
   case 0
-  then have "dom s ={}" using card_eq_0_iff by simp  
+  then have "dom s ={}" using card_eq_0_iff by simp
   then show ?case  by simp
 next
   case (Suc n)
   hence "dom s  \<noteq> {}" using card_gt_0_iff
-    by force 
+    by force
   then obtain x where x_def: "x \<in> dom s" by blast
   then obtain y where y_def: "s x = Some y" by fast
   obtain s' where s'_def: "s' = s(x:=None)" by blast
@@ -1052,9 +1063,9 @@ next
   hence "card (dom s') = n" using x_def Suc by simp
   moreover have "finite (dom s')" using dom' Suc(3) by simp
   ultimately obtain l where "map_of l = s'" using Suc(1) by blast
-  then have "map_of ((x,y)#l) = s" using s'_def y_def by auto 
+  then have "map_of ((x,y)#l) = s" using s'_def y_def by auto
   then show ?case by blast
-qed 
+qed
 qed
 
 lemma map_to_list_id: "finite (dom s) \<Longrightarrow> map_of (map_to_list s) = s "
@@ -1074,10 +1085,10 @@ lemma sas_state_id : "finite (dom x) \<Longrightarrow> sas_state_decode (sas_sta
   apply (auto simp add: map_to_list_id)
   done
 
-  
 
 
-fun imp_assignment_encode:: "vname * bit \<Rightarrow> nat" where 
+
+fun imp_assignment_encode:: "vname * bit \<Rightarrow> nat" where
 "imp_assignment_encode (v,d) = prod_encode (vname_encode v, bit_encode d)"
 
 fun imp_assignment_decode:: "nat \<Rightarrow> (vname * bit)" where
@@ -1101,13 +1112,13 @@ lemma imp_state_id : " finite (dom x) \<Longrightarrow> imp_state_decode (imp_st
     apply (auto simp add: map_to_list_id)
   done
 
-fun comm_imp_state_encode:: "(com * imp_state) \<Rightarrow> nat" where 
+fun comm_imp_state_encode:: "(com * imp_state) \<Rightarrow> nat" where
 "comm_imp_state_encode (c,i) = prod_encode (comm_encode c, imp_state_encode i)"
 
-fun comm_imp_state_decode :: "nat \<Rightarrow> (com*imp_state)" where 
+fun comm_imp_state_decode :: "nat \<Rightarrow> (com*imp_state)" where
 "comm_imp_state_decode n = (case prod_decode n of (c,i) \<Rightarrow> (comm_decode c, imp_state_decode i))"
 
-lemma comm_imp_state_id: 
+lemma comm_imp_state_id:
   "finite (dom (snd x)) \<Longrightarrow> comm_imp_state_decode (comm_imp_state_encode x) = x"
   apply (cases x)
   apply (auto simp only: comm_imp_state_encode.simps comm_imp_state_decode.simps comm_id imp_state_id prod_encode_inverse snd_def)
@@ -1125,11 +1136,11 @@ lemma imp_assignment_list_id: "imp_assignment_list_decode (imp_assignment_list_e
   done
 
 
-fun cilist_encode :: "(com * (vname*bit) list) \<Rightarrow> nat" where 
+fun cilist_encode :: "(com * (vname*bit) list) \<Rightarrow> nat" where
 "cilist_encode (c,i) = prod_encode (comm_encode c, imp_assignment_list_encode i)"
 
-fun cilist_decode :: " nat \<Rightarrow> (com * (vname*bit) list)" where 
-"cilist_decode n = (case prod_decode n of (c,i) \<Rightarrow> 
+fun cilist_decode :: " nat \<Rightarrow> (com * (vname*bit) list)" where
+"cilist_decode n = (case prod_decode n of (c,i) \<Rightarrow>
          (comm_decode c, imp_assignment_list_decode i))"
 
 lemma cilist_id: "cilist_decode(cilist_encode x) = x"
@@ -1157,12 +1168,12 @@ lemma sas_assignment_list_id: "sas_assignment_list_decode (sas_assignment_list_e
   done
 
 
-definition operator_encode :: "operator \<Rightarrow> nat" where 
+definition operator_encode :: "operator \<Rightarrow> nat" where
 "operator_encode op = list_encode [sas_assignment_list_encode (precondition_of op),
                                     sas_assignment_list_encode (effect_of op)] "
 
-definition operator_decode :: " nat \<Rightarrow> operator" where 
-"operator_decode n =  ( case list_decode n of  [p,e] \<Rightarrow> 
+definition operator_decode :: " nat \<Rightarrow> operator" where
+"operator_decode n =  ( case list_decode n of  [p,e] \<Rightarrow>
                        \<lparr>precondition_of = sas_assignment_list_decode p,
                         effect_of = sas_assignment_list_decode e \<rparr> )  "
 
@@ -1180,33 +1191,33 @@ definition list_update_tail :: "nat \<Rightarrow> nat \<Rightarrow> nat \<Righta
 lemma subtail_list_update:
 "list_update_tail l n v = list_update_nat l n v" using list_update_tail_def by auto
 
-lemma sub_list_update : 
+lemma sub_list_update :
       "list_update_nat (list_encode l) n v = list_encode (list_update l n v) "
   apply (induct l arbitrary:n)
   apply (subst list_update_nat.simps)
-  apply (auto simp only: sub_hd sub_head sub_tl sub_cons list_encode_eq split:if_splits list.splits 
+  apply (auto simp only: sub_hd sub_head sub_tl sub_cons list_encode_eq split:if_splits list.splits
             simp flip: list_encode.simps)
   apply ( simp  (no_asm) only: sub_head sub_tail list_encode.simps list_update_def)
   apply simp
    apply simp
   apply (subst list_update_nat.simps)
-   apply (auto simp only: sub_hd sub_head sub_tl sub_cons list_encode_eq split:if_splits list.splits 
+   apply (auto simp only: sub_hd sub_head sub_tl sub_cons list_encode_eq split:if_splits list.splits
             simp flip: list_encode.simps)
    apply simp
   apply (simp only: head.simps sub_cons )
   by (metis One_nat_def Suc_pred list_encode.simps(1) list_update_code(3) neq0_conv sub_cons tail.simps(2))
 
-fun restrict_list :: "('vname,'bit) assignment list \<Rightarrow> 'vname list \<Rightarrow> ('vname,'bit) assignment list" where 
+fun restrict_list :: "('vname,'bit) assignment list \<Rightarrow> 'vname list \<Rightarrow> ('vname,'bit) assignment list" where
 "restrict_list [] s = []" |
 "restrict_list ((x,y)#xs) s = (if x \<in> set s then (x,y) # (restrict_list xs s) else restrict_list xs s)"
 
-lemma sub_restrict_list_helper: 
+lemma sub_restrict_list_helper:
   "map_of (restrict_list xs s) t = restrict_map (map_of xs) (set s) t"
   apply (induct xs)
    apply (auto simp add:snd_def  restrict_map_def)
   done
 
-lemma sub_restrict_list: 
+lemma sub_restrict_list:
 "map_of (restrict_list xs s) = restrict_map (map_of xs) (set s)"
   using sub_restrict_list_helper by fast
 
@@ -1217,10 +1228,10 @@ record  ('variable, 'domain) sas_plus_list_problem =
   goal_ofl :: "('variable, 'domain) assignment list" ("(_\<^sub>G\<^sub>+)" [1000] 999)
   range_ofl :: "('variable, 'domain list) assignment list"
 
-fun vdlist_encode :: "(variable, domain_element list) assignment \<Rightarrow> nat" where 
+fun vdlist_encode :: "(variable, domain_element list) assignment \<Rightarrow> nat" where
 "vdlist_encode (x,y) = prod_encode (variable_encode x,list_encode (map domain_element_encode y))"
 
-fun vdlist_decode ::  "nat \<Rightarrow> (variable, domain_element list) assignment" where 
+fun vdlist_decode ::  "nat \<Rightarrow> (variable, domain_element list) assignment" where
 "vdlist_decode n = (case prod_decode n of (x,y) \<Rightarrow> (variable_decode x, map domain_element_decode (list_decode y)))"
 
 lemma vdlist_id: "vdlist_decode (vdlist_encode x) = x"
@@ -1239,22 +1250,22 @@ fun list_problem_to_problem ::
        \<rparr>"
 
 definition list_problem_encode ::
-    "(variable,domain_element) sas_plus_list_problem \<Rightarrow>nat" where 
+    "(variable,domain_element) sas_plus_list_problem \<Rightarrow>nat" where
 "list_problem_encode x = list_encode [list_encode (map variable_encode (variables_ofl x)),
                                       list_encode (map operator_encode (operators_ofl x)),
                                       sas_assignment_list_encode (initial_ofl x),
                                        sas_assignment_list_encode (goal_ofl x),
                                        list_encode (map vdlist_encode (range_ofl x)) ] "
 
-definition list_problem_decode ::"nat \<Rightarrow> (variable,domain_element) sas_plus_list_problem" where 
-"list_problem_decode x = (case list_decode x of 
+definition list_problem_decode ::"nat \<Rightarrow> (variable,domain_element) sas_plus_list_problem" where
+"list_problem_decode x = (case list_decode x of
 [var,op,i,g,r]  \<Rightarrow> \<lparr>           variables_ofl = map variable_decode (list_decode var),
                                operators_ofl = map operator_decode (list_decode op),
                                initial_ofl = sas_assignment_list_decode i,
                                goal_ofl = sas_assignment_list_decode g,
                                range_ofl = map vdlist_decode (list_decode r) \<rparr> )"
 
-lemma list_problem_id : 
+lemma list_problem_id :
       "list_problem_decode (list_problem_encode x) = x"
   apply (auto simp only:list_problem_encode_def list_problem_decode_def list_encode_inverse)
   apply (auto simp add: comp_def variable_id operator_id sas_assignment_list_id vdlist_id simp del: vdlist_decode.simps)
@@ -1262,12 +1273,12 @@ lemma list_problem_id :
 
 declare elemof.simps [simp del]
 
-fun restrict_nat :: "nat \<Rightarrow> nat \<Rightarrow> nat" where 
-"restrict_nat l s = (if l = 0 then 0 else (let t = restrict_nat (tl_nat l) s in (if elemof (fst_nat (hd_nat l)) s \<noteq> 0 then 
+fun restrict_nat :: "nat \<Rightarrow> nat \<Rightarrow> nat" where
+"restrict_nat l s = (if l = 0 then 0 else (let t = restrict_nat (tl_nat l) s in (if elemof (fst_nat (hd_nat l)) s \<noteq> 0 then
     (hd_nat l)## t else t))) "
 
-fun restrict_acc :: "nat \<Rightarrow> nat \<Rightarrow> nat \<Rightarrow> nat" where 
-"restrict_acc acc l s = (if l = 0 then acc else(if elemof (fst_nat (hd_nat l)) s \<noteq> 0 then 
+fun restrict_acc :: "nat \<Rightarrow> nat \<Rightarrow> nat \<Rightarrow> nat" where
+"restrict_acc acc l s = (if l = 0 then acc else(if elemof (fst_nat (hd_nat l)) s \<noteq> 0 then
    restrict_acc  ((hd_nat l)## acc) (tl_nat l) s else restrict_acc acc (tl_nat l) s)) "
 
 lemma sub_restrict_nat:
@@ -1278,13 +1289,13 @@ lemma sub_restrict_nat:
   subgoal for x l
     apply (cases x)
   apply (subst restrict_nat.simps)
-    apply (auto simp only:  sub_cons restrict_list.simps list_encode_eq sub_tl  imp_assignment_list_encode_def sub_tail_map Let_def sub_fst sub_hd sub_head_map list.simps  head.simps imp_assignment_encode.simps fst_def tail.simps non_empty_positive  split:if_splits 
-  simp flip: list_encode.simps 
+    apply (auto simp only:  sub_cons restrict_list.simps list_encode_eq sub_tl  imp_assignment_list_encode_def sub_tail_map Let_def sub_fst sub_hd sub_head_map list.simps  head.simps imp_assignment_encode.simps fst_def tail.simps non_empty_positive  split:if_splits
+  simp flip: list_encode.simps
 )
      apply (auto simp only: list_encode.simps sub_elem_of2)
      apply simp
     apply (metis imageE set_map vname_id)
-    done    
+    done
   done
 
 lemma sub_restrict_nat_gen:
@@ -1294,8 +1305,8 @@ lemma sub_restrict_nat_gen:
   subgoal for x xs
   apply (cases x)
   apply (subst restrict_nat.simps)
-    apply (auto simp only:  sub_cons restrict_list.simps list_encode_eq sub_tl  imp_assignment_list_encode_def sub_tail_map Let_def sub_fst sub_hd sub_head_map list.simps  head.simps imp_assignment_encode.simps fst_def tail.simps non_empty_positive  split:if_splits 
-  simp flip: list_encode.simps 
+    apply (auto simp only:  sub_cons restrict_list.simps list_encode_eq sub_tl  imp_assignment_list_encode_def sub_tail_map Let_def sub_fst sub_hd sub_head_map list.simps  head.simps imp_assignment_encode.simps fst_def tail.simps non_empty_positive  split:if_splits
+  simp flip: list_encode.simps
 )
      apply (auto simp only: list_encode.simps sub_elem_of2)
     done
@@ -1319,13 +1330,13 @@ proof -
     done
 qed
 
-definition restrict_tail :: "nat \<Rightarrow> nat \<Rightarrow> nat " where 
+definition restrict_tail :: "nat \<Rightarrow> nat \<Rightarrow> nat " where
 "restrict_tail l s = reverse_nat (restrict_acc 0 l s)"
 
-lemma subtail_restrict: 
+lemma subtail_restrict:
 "restrict_tail l s =  restrict_nat l s"
   using append_nat_0 restrict_induct restrict_tail_def rev_rev_nat by auto
-  
+
 declare elemof.simps [simp]
 
 
@@ -1333,11 +1344,11 @@ declare elemof.simps [simp]
 type_synonym  var = "variable SAS_Plus_Plus_To_SAS_Plus.variable"
 type_synonym  dom = "domain_element SAS_Plus_Plus_To_SAS_Plus.domain_element"
 type_synonym  sas_plus_state = "(var,dom)  State_Variable_Representation.state"
-fun var_encode :: "var \<Rightarrow> nat" where 
+fun var_encode :: "var \<Rightarrow> nat" where
 "var_encode Stage = 0 " |
 "var_encode (Var v) = Suc (variable_encode v)"
 
-fun var_decode :: "nat \<Rightarrow> var" where 
+fun var_decode :: "nat \<Rightarrow> var" where
 "var_decode 0 = Stage"|
 "var_decode (Suc v) = (Var (variable_decode v))"
 
@@ -1346,12 +1357,12 @@ lemma var_id: "var_decode (var_encode x) = x"
    apply (auto simp add:variable_id)
   done
 
-fun dom_encode :: "dom \<Rightarrow> nat" where 
+fun dom_encode :: "dom \<Rightarrow> nat" where
 "dom_encode NonInit = 0"|
 "dom_encode Init = Suc 0"|
 "dom_encode (DE d) = Suc (Suc (domain_element_encode d))"
 
-fun dom_decode :: "nat \<Rightarrow> dom" where 
+fun dom_decode :: "nat \<Rightarrow> dom" where
 "dom_decode 0 = NonInit"|
 "dom_decode (Suc 0) = Init"|
 "dom_decode (Suc (Suc d)) = DE (domain_element_decode d)"
@@ -1361,14 +1372,14 @@ lemma dom_id : "dom_decode (dom_encode x) = x"
    apply (auto simp add:domain_element_id simp del: domain_element_decode.simps)
   done
 
-fun sas_plus_assignment_encode:: "(var,dom) assignment \<Rightarrow> nat" where 
+fun sas_plus_assignment_encode:: "(var,dom) assignment \<Rightarrow> nat" where
   "sas_plus_assignment_encode (v,d) = prod_encode(var_encode v, dom_encode d)"
 
-fun sas_plus_assignment_decode:: " nat \<Rightarrow> (var,dom) assignment" where 
-  "sas_plus_assignment_decode n = (case prod_decode n of (v,d) \<Rightarrow> 
+fun sas_plus_assignment_decode:: " nat \<Rightarrow> (var,dom) assignment" where
+  "sas_plus_assignment_decode n = (case prod_decode n of (v,d) \<Rightarrow>
                                 (var_decode v, dom_decode d))"
 
-lemma sas_plus_assignment_id: 
+lemma sas_plus_assignment_id:
       "sas_plus_assignment_decode (sas_plus_assignment_encode x) = x"
   apply (cases x)
   apply (auto simp add:var_id dom_id)
@@ -1386,11 +1397,11 @@ lemma sas_plus_assignment_list_id:
         sas_plus_assignment_id  simp del: sas_plus_assignment_decode.simps)
   done
 
-fun islist_encode :: "(dom \<times> (variable,domain_element) assignment list) \<Rightarrow> nat" where 
+fun islist_encode :: "(dom \<times> (variable,domain_element) assignment list) \<Rightarrow> nat" where
 "islist_encode (i,s) = prod_encode (dom_encode i, sas_assignment_list_encode s)"
 
-fun islist_decode :: "nat \<Rightarrow> (dom \<times> (variable,domain_element) assignment list)" where 
-"islist_decode n = (case prod_decode n of (i,s) \<Rightarrow> 
+fun islist_decode :: "nat \<Rightarrow> (dom \<times> (variable,domain_element) assignment list)" where
+"islist_decode n = (case prod_decode n of (i,s) \<Rightarrow>
          (dom_decode i, sas_assignment_list_decode s))"
 
 lemma islist_id: "islist_decode(islist_encode x) = x"
@@ -1407,12 +1418,12 @@ definition sas_plus_state_decode :: "nat \<Rightarrow> sas_plus_state" where
 type_synonym operator_plus = "(var, dom) sas_plus_operator"
 type_synonym problem_plus = "(var, dom) sas_plus_problem"
 
-definition operator_plus_encode :: "operator_plus \<Rightarrow> nat" where 
+definition operator_plus_encode :: "operator_plus \<Rightarrow> nat" where
 "operator_plus_encode op = list_encode [sas_plus_assignment_list_encode (precondition_of op),
                                     sas_plus_assignment_list_encode (effect_of op)] "
 
-definition operator_plus_decode :: " nat \<Rightarrow> operator_plus" where 
-"operator_plus_decode n =  ( case list_decode n of  [p,e] \<Rightarrow> 
+definition operator_plus_decode :: " nat \<Rightarrow> operator_plus" where
+"operator_plus_decode n =  ( case list_decode n of  [p,e] \<Rightarrow>
                        \<lparr>precondition_of = sas_plus_assignment_list_decode p,
                         effect_of = sas_plus_assignment_list_decode e \<rparr> )  "
 
@@ -1420,14 +1431,14 @@ lemma operator_plus_id : " operator_plus_decode (operator_plus_encode x) = x"
   apply (auto simp add:operator_plus_decode_def operator_plus_encode_def sas_plus_assignment_list_id)
   done
 
-fun the_nat :: "nat \<Rightarrow> nat" where 
+fun the_nat :: "nat \<Rightarrow> nat" where
  "the_nat x = x-1"
 
-fun list_option_encode :: " nat list option \<Rightarrow> nat" where 
+fun list_option_encode :: " nat list option \<Rightarrow> nat" where
 "list_option_encode None = 0"|
 "list_option_encode (Some x) = Suc (list_encode x)"
 
-fun list_option_decode :: "nat \<Rightarrow>  nat list option" where 
+fun list_option_decode :: "nat \<Rightarrow>  nat list option" where
 "list_option_decode 0 = None"|
 "list_option_decode (Suc x) = Some (list_decode x)"
 
@@ -1439,17 +1450,17 @@ lemma list_option_id:"list_option_decode (list_option_encode x) = x"
 lemma sub_the: " the_nat (list_option_encode x) = list_encode (thef x)"
   apply (cases x)
    apply (auto)
-  done  
+  done
 
-fun thefn :: "nat option \<Rightarrow> nat" where 
+fun thefn :: "nat option \<Rightarrow> nat" where
 "thefn None = 0"|
 "thefn (Some x) = x"
 
-lemma sub_the2: "the_nat (option_encode  x) = thefn x" 
+lemma sub_the2: "the_nat (option_encode  x) = thefn x"
   apply (cases x)
   apply auto
   done
-  
+
 
 fun map_list_find ::"('a,'b) assignment list \<Rightarrow>'a \<Rightarrow> 'b option" where
 "map_list_find [] _ = None "|
@@ -1460,8 +1471,8 @@ lemma sub_map_list_find: "map_list_find xs a = (map_of xs) a"
    apply auto
   done
 
-fun map_list_find_nat :: "nat \<Rightarrow> nat \<Rightarrow> nat" where 
-"map_list_find_nat xs a = (if xs = 0 then 0 else if fst_nat (hd_nat xs) = a then some_nat (snd_nat (hd_nat xs))  
+fun map_list_find_nat :: "nat \<Rightarrow> nat \<Rightarrow> nat" where
+"map_list_find_nat xs a = (if xs = 0 then 0 else if fst_nat (hd_nat xs) = a then some_nat (snd_nat (hd_nat xs))
   else map_list_find_nat (tl_nat xs) a) "
 
 lemma sub_map_list_find_nat:
@@ -1475,10 +1486,10 @@ lemma sub_map_list_find_nat:
   apply auto
   done
 
-fun vdlist_plus_encode :: "(var, dom list) assignment \<Rightarrow> nat" where 
+fun vdlist_plus_encode :: "(var, dom list) assignment \<Rightarrow> nat" where
 "vdlist_plus_encode (x,y) = prod_encode (var_encode x,list_encode (map dom_encode y))"
 
-fun vdlist_plus_decode ::  "nat \<Rightarrow> (var, dom list) assignment" where 
+fun vdlist_plus_decode ::  "nat \<Rightarrow> (var, dom list) assignment" where
 "vdlist_plus_decode n = (case prod_decode n of (x,y) \<Rightarrow> (var_decode x, map dom_decode (list_decode y)))"
 
 lemma vdlist_plus_id: "vdlist_plus_decode (vdlist_plus_encode x) = x"
@@ -1487,22 +1498,22 @@ lemma vdlist_plus_id: "vdlist_plus_decode (vdlist_plus_encode x) = x"
   done
 
 definition list_problem_plus_encode ::
-    "(var,dom) sas_plus_list_problem \<Rightarrow>nat" where 
+    "(var,dom) sas_plus_list_problem \<Rightarrow>nat" where
 "list_problem_plus_encode x = list_encode [list_encode (map var_encode (variables_ofl x)),
                                       list_encode (map operator_plus_encode (operators_ofl x)),
                                       sas_plus_assignment_list_encode (initial_ofl x),
                                        sas_plus_assignment_list_encode (goal_ofl x),
                                        list_encode (map vdlist_plus_encode (range_ofl x)) ] "
 
-definition list_problem_plus_decode ::"nat \<Rightarrow> (var,dom) sas_plus_list_problem" where 
-"list_problem_plus_decode x = (case list_decode x of 
+definition list_problem_plus_decode ::"nat \<Rightarrow> (var,dom) sas_plus_list_problem" where
+"list_problem_plus_decode x = (case list_decode x of
 [var,op,i,g,r]  \<Rightarrow> \<lparr>           variables_ofl = map var_decode (list_decode var),
                                operators_ofl = map operator_plus_decode (list_decode op),
                                initial_ofl = sas_plus_assignment_list_decode i,
                                goal_ofl = sas_plus_assignment_list_decode g,
                                range_ofl = map vdlist_plus_decode (list_decode r) \<rparr> )"
 
-lemma list_problem_plus_id : 
+lemma list_problem_plus_id :
       "list_problem_plus_decode (list_problem_plus_encode x) = x"
   apply (auto simp only:list_problem_plus_encode_def list_problem_plus_decode_def list_encode_inverse)
   apply (auto simp add: comp_def var_id operator_plus_id sas_plus_assignment_list_id vdlist_plus_id simp del: vdlist_plus_decode.simps)
@@ -1515,10 +1526,10 @@ lemma sub_thefn: "the_nat (option_encode x) =thefn x"
    apply (auto)
   done
 
-definition fun_of :: "(vname,nat) assignment list \<Rightarrow> vname \<Rightarrow> nat" where 
+definition fun_of :: "(vname,nat) assignment list \<Rightarrow> vname \<Rightarrow> nat" where
 "fun_of x v =  (case (map_of x) v of None \<Rightarrow> 0 | Some x \<Rightarrow> x)"
 
-fun fun_list_find :: "('a,nat) assignment list \<Rightarrow> 'a \<Rightarrow> nat" where 
+fun fun_list_find :: "('a,nat) assignment list \<Rightarrow> 'a \<Rightarrow> nat" where
 "fun_list_find [] _ = 0"|
 "fun_list_find ((x,y)#xs) a = (if x= a then y else fun_list_find xs a)"
 
@@ -1527,10 +1538,10 @@ lemma sub_fun_list_find:"fun_list_find xs a = fun_of xs a"
    apply (auto simp add:fun_of_def)
   done
 
-fun fun_list_find_nat :: "nat \<Rightarrow> nat \<Rightarrow> nat" where 
+fun fun_list_find_nat :: "nat \<Rightarrow> nat \<Rightarrow> nat" where
 "fun_list_find_nat xs a  = (if xs = 0 then 0 else if fst_nat (hd_nat xs) = a then snd_nat (hd_nat xs) else fun_list_find_nat (tl_nat xs) a) "
 
-fun fun_list_find_tail :: "nat \<Rightarrow> nat \<Rightarrow> nat" where 
+fun fun_list_find_tail :: "nat \<Rightarrow> nat \<Rightarrow> nat" where
 "fun_list_find_tail xs a  = (if xs = 0 then 0 else if fst_nat (hd_nat xs) = a then snd_nat (hd_nat xs) else fun_list_find_tail (tl_nat xs) a) "
 
 lemma subtail_fun_list_find: "fun_list_find_tail xs a = fun_list_find_nat xs a"
@@ -1543,42 +1554,42 @@ lemma sub_fun_list_find_nat :
   apply (induct xs)
    apply simp
   apply (subst fun_list_find_nat.simps)
-  apply (auto simp only: list.simps list_encode_eq 
-        sub_hd head.simps sub_fst fst_def sub_snd snd_def sub_tl tail.simps 
+  apply (auto simp only: list.simps list_encode_eq
+        sub_hd head.simps sub_fst fst_def sub_snd snd_def sub_tl tail.simps
 
 simp flip: list_encode.simps
-        
+
  )
   apply auto
   done
 
-fun impm_assignment_encode :: "(vname,nat) assignment \<Rightarrow> nat" where 
+fun impm_assignment_encode :: "(vname,nat) assignment \<Rightarrow> nat" where
 "impm_assignment_encode (v,n) = prod_encode (vname_encode v, n)"
 
-fun impm_assignment_decode :: " nat \<Rightarrow> (vname,nat) assignment" where 
+fun impm_assignment_decode :: " nat \<Rightarrow> (vname,nat) assignment" where
 "impm_assignment_decode  x =  (case prod_decode x of (v,n) \<Rightarrow> (vname_decode v, n))"
 
 lemma impm_assignment_id:"impm_assignment_decode (impm_assignment_encode x) = x"
   by (cases x) (auto simp add:vname_id)
 
-definition impm_assignment_list_encode ::  "(vname,nat) assignment list \<Rightarrow> nat" where 
+definition impm_assignment_list_encode ::  "(vname,nat) assignment list \<Rightarrow> nat" where
 "impm_assignment_list_encode x = list_encode (map impm_assignment_encode x)"
 
-definition impm_assignment_list_decode ::  "nat \<Rightarrow> (vname,nat) assignment list" where 
+definition impm_assignment_list_decode ::  "nat \<Rightarrow> (vname,nat) assignment list" where
 "impm_assignment_list_decode x = map impm_assignment_decode ( list_decode x)"
 
-lemma impm_assignment_list_id: 
+lemma impm_assignment_list_id:
   "impm_assignment_list_decode (impm_assignment_list_encode x) = x"
   apply (auto simp add: impm_assignment_list_decode_def  impm_assignment_list_encode_def)
   apply (auto simp only: comp_def impm_assignment_id)
   apply auto
   done
 
-fun bit_option_encode :: "bit option \<Rightarrow> nat" where 
+fun bit_option_encode :: "bit option \<Rightarrow> nat" where
 "bit_option_encode None = 0"|
 "bit_option_encode (Some x) = Suc (bit_encode x)"
 
-fun bit_option_decode :: "nat \<Rightarrow> bit option" where 
+fun bit_option_decode :: "nat \<Rightarrow> bit option" where
 "bit_option_decode 0 = None"|
 "bit_option_decode (Suc n ) = Some (bit_decode n)"
 
@@ -1601,14 +1612,14 @@ fun_list_find (map (\<lambda>(x,y). (x , g y)) xs) x
    apply (auto simp add:inj_def)
   done
 
-fun max_list :: "nat list \<Rightarrow> nat" where 
+fun max_list :: "nat list \<Rightarrow> nat" where
 "max_list [] = 0"|
 "max_list (x#xs) = max x (max_list xs)"
 
-fun max_list_nat :: "nat \<Rightarrow> nat" where 
+fun max_list_nat :: "nat \<Rightarrow> nat" where
 "max_list_nat xs = (if xs = 0 then 0 else max (hd_nat xs) (max_list_nat (tl_nat xs)))"
 
-fun max_list_acc :: "nat \<Rightarrow> nat \<Rightarrow> nat" where 
+fun max_list_acc :: "nat \<Rightarrow> nat \<Rightarrow> nat" where
 "max_list_acc acc xs = (if xs = 0 then acc else max_list_acc (max (hd_nat xs) acc) (tl_nat xs))"
 
 lemma sub_max_list_nat: "max_list_nat (list_encode xs) = max_list xs"
@@ -1633,13 +1644,13 @@ proof -
     done
 qed
 
-definition max_list_tail :: "nat \<Rightarrow>  nat" where 
+definition max_list_tail :: "nat \<Rightarrow>  nat" where
 "max_list_tail xs = max_list_acc 0 xs "
 
-lemma subtail_max_list: 
+lemma subtail_max_list:
 "max_list_tail xs =  max_list_nat xs"
   using max_list_acc_correct max_list_tail_def by presburger
-  
+
 
 
 lemma sub_max_list: "xs \<noteq> [] \<Longrightarrow> max_list xs = Max (set xs)"
@@ -1649,11 +1660,11 @@ lemma sub_max_list: "xs \<noteq> [] \<Longrightarrow> max_list xs = Max (set xs)
    apply (auto)
   using Max_insert
   by (metis List.finite_set Max_singleton empty_iff list.set(1) list.set_intros(1)
- list.simps(15) max_0R max_list.elims) 
+ list.simps(15) max_0R max_list.elims)
 
 
 
-fun del :: "('a,'b) assignment list \<Rightarrow> 'a \<Rightarrow>  ('a,'b) assignment list" where 
+fun del :: "('a,'b) assignment list \<Rightarrow> 'a \<Rightarrow>  ('a,'b) assignment list" where
 "del [] _ = []"|
 "del ((x,y)#xs) a = (if x = a then del xs a else (x,y)# del xs a)"
 
@@ -1664,7 +1675,7 @@ lemma del_filter:
   done
 
 
-fun del_nat :: "nat \<Rightarrow> nat \<Rightarrow> nat" where 
+fun del_nat :: "nat \<Rightarrow> nat \<Rightarrow> nat" where
 "del_nat xs a = (if xs =0 then 0 else if fst_nat (hd_nat xs) = a then del_nat (tl_nat xs) a else cons
 (hd_nat xs)  (del_nat (tl_nat xs) a) )"
 lemma sub_del: "del_nat (list_encode (map prod_encode xs)) a = list_encode (map prod_encode (del xs a))"
@@ -1692,7 +1703,7 @@ lemma del_correct_corr: " a \<noteq> x \<Longrightarrow> map_of (del xs a) x = m
   apply (induct xs)
    apply (auto split:if_splits)
   done
-fun nub :: "('a,'b) assignment list \<Rightarrow> ('a,'b) assignment list" where 
+fun nub :: "('a,'b) assignment list \<Rightarrow> ('a,'b) assignment list" where
 "nub [] = [] "|
 "nub ((x,y)#xs) = (x,y) # nub (del xs x) "
 
@@ -1701,7 +1712,7 @@ lemma del_shorter : "length (del xs a) \<le> length xs"
    apply auto
   done
 
-function nub_nat :: "nat \<Rightarrow> nat" where 
+function nub_nat :: "nat \<Rightarrow> nat" where
 "nub_nat xs = (if xs = 0 then 0 else (hd_nat xs) ## nub_nat (del_nat xs (fst_nat (hd_nat xs))))"
   by pat_completeness auto
 termination
@@ -1743,13 +1754,13 @@ lemma nub_includes: "set (nub xs) \<subseteq> set xs"
   apply (induct xs rule: nub.induct)
    apply (auto)
   using del_includes apply fast
-   using del_includes apply fast  
+   using del_includes apply fast
   done
-  
+
 lemma nub_correct : "distinct (map fst (nub xs))"
   apply (induct xs rule:nub.induct)
    apply auto
-  using nub_includes del_correct by fastforce 
+  using nub_includes del_correct by fastforce
 
 lemma map_of_nub_apply:"map_of (nub xs) x = map_of xs x"
   apply (induct xs rule:nub.induct)
@@ -1759,10 +1770,10 @@ lemma map_of_nub:"map_of (nub xs)  = map_of xs "
   using map_of_nub_apply by fast
 
 
-definition ran_list :: "('a,'b) assignment list \<Rightarrow> 'b list" where 
+definition ran_list :: "('a,'b) assignment list \<Rightarrow> 'b list" where
 "ran_list xs = map snd (nub xs)"
 
-fun map_snd  :: "nat \<Rightarrow> nat " where 
+fun map_snd  :: "nat \<Rightarrow> nat " where
 "map_snd xs = (if xs = 0 then 0 else (snd_nat (hd_nat xs)) ## map_snd (tl_nat xs))"
 
 lemma submap_snd:
@@ -1771,7 +1782,7 @@ lemma submap_snd:
   apply auto
   done
 
-definition ran_nat :: "nat \<Rightarrow> nat" where 
+definition ran_nat :: "nat \<Rightarrow> nat" where
 "ran_nat xs = map_snd (nub_nat xs)"
 
 lemma sub_ran_nat : "ran_nat (list_encode (map prod_encode  xs)) = list_encode (ran_list xs) "
@@ -1779,7 +1790,7 @@ lemma sub_ran_nat : "ran_nat (list_encode (map prod_encode  xs)) = list_encode (
  sub_nub sub_map map_map comp_def sub_snd)
   done
 
-lemma sub_ran_list_helper : "distinct (map fst xs) \<Longrightarrow> 
+lemma sub_ran_list_helper : "distinct (map fst xs) \<Longrightarrow>
 set (map snd xs) = ran (map_of xs)"
   apply (induct xs)
    apply (auto)
@@ -1788,7 +1799,7 @@ set (map snd xs) = ran (map_of xs)"
   done
 
 lemma sub_ran_list : "set (ran_list xs) = ran (map_of xs)"
-  apply (simp only:ran_list_def sub_ran_list_helper[of "nub xs"] nub_correct[of xs] map_of_nub ) 
+  apply (simp only:ran_list_def sub_ran_list_helper[of "nub xs"] nub_correct[of xs] map_of_nub )
   done
 
 lemma ran_list_pre:"I \<noteq> [] \<Longrightarrow> ran_list I \<noteq> []"
@@ -1819,7 +1830,7 @@ lemma sub_restrict_apply: "map_of (map (\<lambda>(x,y). (x, the y)) (filter (\<l
 lemma sub_restrict: "map_of (map (\<lambda>(x,y). (x, the y)) (filter (\<lambda>(x,y) . y \<noteq> None) (map (\<lambda>x. (x,f x)) xs))) = (f |` set xs) "
   using sub_restrict_apply by fast
 
-fun filter_nat ::"(nat\<Rightarrow> bool) \<Rightarrow> nat \<Rightarrow> nat" where 
+fun filter_nat ::"(nat\<Rightarrow> bool) \<Rightarrow> nat \<Rightarrow> nat" where
 "filter_nat f xs = (if xs = 0 then 0 else if f (hd_nat xs) then (hd_nat xs) ## (filter_nat f (tl_nat xs)) else (filter_nat f (tl_nat xs))) "
 
 lemma sub_filter: "filter_nat f (list_encode xs) = list_encode (filter f xs)"
@@ -1838,7 +1849,7 @@ lemma sub_restrict_map_nat: "map_nat (\<lambda>n. prod_encode(fst_nat n, the_nat
   apply (auto simp add: sub_snd list_encode_eq sub_fst simp del: list_encode.simps)
   using option_encode.elims by blast
 
-fun bit_option_to_option ::"bit option \<Rightarrow> nat option" where 
+fun bit_option_to_option ::"bit option \<Rightarrow> nat option" where
 "bit_option_to_option None = None"|
 "bit_option_to_option (Some x) = Some (bit_encode x)"
 
@@ -1866,22 +1877,22 @@ lemma map_list_find_map_none: "( map_list_find (map (\<lambda>(x,y). (x , f y)) 
    apply auto
   done
 
-fun bool_encode :: "bool \<Rightarrow> nat" where 
+fun bool_encode :: "bool \<Rightarrow> nat" where
 "bool_encode False = 0"|
 "bool_encode True = 1"
 
-fun bool_decode :: "nat \<Rightarrow> bool" where 
+fun bool_decode :: "nat \<Rightarrow> bool" where
 "bool_decode 0 = False"|
 "bool_decode (Suc x ) = True"
 
 lemma bool_id : "bool_decode (bool_encode x) = x"
   by (cases x) auto
 
-fun strips_assignment_encode :: "((var,dom) assignment,bool) assignment \<Rightarrow> nat" where 
+fun strips_assignment_encode :: "((var,dom) assignment,bool) assignment \<Rightarrow> nat" where
 "strips_assignment_encode (s,b) = prod_encode (sas_plus_assignment_encode s , bool_encode b)"
 
-fun strips_assignment_decode :: "nat \<Rightarrow> ((var,dom) assignment,bool) assignment" where 
-"strips_assignment_decode n = (case prod_decode n of (s,b) \<Rightarrow> 
+fun strips_assignment_decode :: "nat \<Rightarrow> ((var,dom) assignment,bool) assignment" where
+"strips_assignment_decode n = (case prod_decode n of (s,b) \<Rightarrow>
 (sas_plus_assignment_decode s , bool_decode b))"
 
 lemma strips_assignment_id : "strips_assignment_decode (strips_assignment_encode x) = x"
@@ -1889,10 +1900,10 @@ lemma strips_assignment_id : "strips_assignment_decode (strips_assignment_encode
   apply (auto simp add:var_id dom_id bool_id)
   done
 
-definition strips_assignment_list_encode :: "((var,dom) assignment,bool) assignment list \<Rightarrow> nat" where 
+definition strips_assignment_list_encode :: "((var,dom) assignment,bool) assignment list \<Rightarrow> nat" where
 "strips_assignment_list_encode  x = list_encode (map strips_assignment_encode x)"
 
-definition strips_assignment_list_decode :: "nat \<Rightarrow> ((var,dom) assignment,bool) assignment list" where 
+definition strips_assignment_list_decode :: "nat \<Rightarrow> ((var,dom) assignment,bool) assignment list" where
 "strips_assignment_list_decode  x = map strips_assignment_decode (list_decode x)"
 
 lemma strips_assignment_list_id: "strips_assignment_list_decode (strips_assignment_list_encode x) = x"
@@ -1924,23 +1935,23 @@ lemma snd_sas_simp : "snd_nat (sas_plus_assignment_encode x ) = dom_encode (snd 
   apply (auto simp add:sub_snd)
   done
 
-    
+
 lemma dom_inj : "inj dom_encode"
   apply (auto simp add:inj_def)
   by (metis dom_id)
-    
+
 lemma dom_inj_simp : "(dom_encode a = dom_encode b) = (a=b)"
   using dom_inj inj_def by metis
 
-fun strips_operator_encode :: "(var,dom) assignment strips_operator \<Rightarrow> nat" where 
+fun strips_operator_encode :: "(var,dom) assignment strips_operator \<Rightarrow> nat" where
 "strips_operator_encode op = list_encode [sas_plus_assignment_list_encode (strips_operator.precondition_of op),
                                          sas_plus_assignment_list_encode (strips_operator.add_effects_of op),
                                          sas_plus_assignment_list_encode (strips_operator.delete_effects_of op)]"
 
 
-fun strips_operator_decode :: "nat \<Rightarrow> (var,dom) assignment strips_operator " where 
+fun strips_operator_decode :: "nat \<Rightarrow> (var,dom) assignment strips_operator " where
 "strips_operator_decode n = (case list_decode n of [pre,add,delete] \<Rightarrow>
-      \<lparr>strips_operator.precondition_of = sas_plus_assignment_list_decode pre, 
+      \<lparr>strips_operator.precondition_of = sas_plus_assignment_list_decode pre,
         strips_operator.add_effects_of =  sas_plus_assignment_list_decode add,
         strips_operator.delete_effects_of =  sas_plus_assignment_list_decode delete \<rparr>)
 "
@@ -1956,8 +1967,8 @@ record  ('variable) strips_list_problem =
   goal_of :: "('variable,bool) assignment list" ("(_\<^sub>G)" [1000] 999)
 
 fun strips_list_problem_to_problem ::
- "('variable) strips_list_problem \<Rightarrow> ('variable)strips_problem" where 
-"strips_list_problem_to_problem P = 
+ "('variable) strips_list_problem \<Rightarrow> ('variable)strips_problem" where
+"strips_list_problem_to_problem P =
 \<lparr>
   strips_problem.variables_of = variables_of P,
   operators_of = operators_of P,
@@ -1965,28 +1976,28 @@ fun strips_list_problem_to_problem ::
   goal_of = map_of (goal_of P)
  \<rparr>"
 
-definition strips_operator_list_encode :: " (var,dom) assignment strips_operator list \<Rightarrow> nat" where 
+definition strips_operator_list_encode :: " (var,dom) assignment strips_operator list \<Rightarrow> nat" where
 " strips_operator_list_encode xs = list_encode (map  strips_operator_encode xs)"
 
-definition strips_operator_list_decode :: " nat \<Rightarrow> (var,dom) assignment strips_operator list" where 
+definition strips_operator_list_decode :: " nat \<Rightarrow> (var,dom) assignment strips_operator list" where
 " strips_operator_list_decode n = map  strips_operator_decode (list_decode n)"
 
 lemma strips_operator_list_id:
 "  strips_operator_list_decode ( strips_operator_list_encode x) = x"
   apply (auto simp only:  strips_operator_list_decode_def  strips_operator_list_encode_def
 comp_def list_encode_inverse map_map strips_operator_id)
-  apply auto 
+  apply auto
   done
 
-fun strips_list_problem_encode :: "((var,dom) assignment) strips_list_problem \<Rightarrow> nat" where 
-"strips_list_problem_encode P = list_encode 
+fun strips_list_problem_encode :: "((var,dom) assignment) strips_list_problem \<Rightarrow> nat" where
+"strips_list_problem_encode P = list_encode
 [sas_plus_assignment_list_encode(variables_of P),
 strips_operator_list_encode (operators_of P),
 strips_assignment_list_encode (initial_of P),
 strips_assignment_list_encode (goal_of P)
 ]"
 
-fun strips_list_problem_decode :: "nat \<Rightarrow> ((var,dom) assignment) strips_list_problem" where 
+fun strips_list_problem_decode :: "nat \<Rightarrow> ((var,dom) assignment) strips_list_problem" where
 "strips_list_problem_decode n = (case list_decode n of
 [vs,ops,I,gs] \<Rightarrow> \<lparr>
   variables_of  = sas_plus_assignment_list_decode vs,
@@ -2000,11 +2011,11 @@ lemma  strips_list_problem_id:
   apply (auto simp add:sas_plus_assignment_list_id strips_operator_list_id strips_assignment_list_id )
   done
 
-fun sat_variable_encode :: "sat_plan_variable \<Rightarrow> nat" where 
+fun sat_variable_encode :: "sat_plan_variable \<Rightarrow> nat" where
 "sat_variable_encode (State x y) = list_encode [0,x,y]"|
 "sat_variable_encode (Operator x y) = list_encode [1,x,y]"
 
-fun sat_variable_decode :: "nat \<Rightarrow> sat_plan_variable" where 
+fun sat_variable_decode :: "nat \<Rightarrow> sat_plan_variable" where
 "sat_variable_decode n = (case list_decode n of [0,x,y] \<Rightarrow> State x y | [Suc 0, x ,y] \<Rightarrow> Operator x y)"
 
 lemma sat_variable_id :
@@ -2013,7 +2024,7 @@ lemma sat_variable_id :
    apply (auto)
   done
 
-fun sat_formula_encode :: "sat_plan_formula \<Rightarrow> nat" where 
+fun sat_formula_encode :: "sat_plan_formula \<Rightarrow> nat" where
 "sat_formula_encode Bot = list_encode [0] "|
 "sat_formula_encode (Atom v) = list_encode [1, sat_variable_encode v] "|
 "sat_formula_encode (Not v) = list_encode[2, sat_formula_encode v]"|
@@ -2021,7 +2032,7 @@ fun sat_formula_encode :: "sat_plan_formula \<Rightarrow> nat" where
 "sat_formula_encode (Or a b) = list_encode[4,sat_formula_encode a,sat_formula_encode b]"|
 "sat_formula_encode (Imp a b) = list_encode[5,sat_formula_encode a,sat_formula_encode b]"
 
-fun sat_formula_decode :: "nat \<Rightarrow> sat_plan_formula" where 
+fun sat_formula_decode :: "nat \<Rightarrow> sat_plan_formula" where
 "sat_formula_decode n =  (case list_decode n of
   [0] \<Rightarrow> Bot|
   [Suc 0,v] \<Rightarrow> Atom (sat_variable_decode v)|
@@ -2031,17 +2042,17 @@ fun sat_formula_decode :: "nat \<Rightarrow> sat_plan_formula" where
   [Suc (Suc (Suc (Suc (Suc 0)))),a,b] \<Rightarrow> Imp (sat_formula_decode a) (sat_formula_decode b)
 ) "
 
-lemma sat_formula_id : 
+lemma sat_formula_id :
 "sat_formula_decode (sat_formula_encode x) = x"
   apply (induct x)
   apply (auto simp add: sat_variable_id simp del: sat_variable_decode.simps)
   done
 
-fun bool_option_encode :: "bool option \<Rightarrow> nat" where 
+fun bool_option_encode :: "bool option \<Rightarrow> nat" where
 "bool_option_encode None = 0"|
 "bool_option_encode (Some b) = Suc (bool_encode b)"
 
-fun bool_option_decode :: "nat \<Rightarrow> bool option" where 
+fun bool_option_decode :: "nat \<Rightarrow> bool option" where
 "bool_option_decode 0 = None"|
 "bool_option_decode (Suc b) = Some (bool_decode b)"
 
@@ -2051,7 +2062,7 @@ lemma bool_option_id :
    apply (auto simp add:bool_id)
   done
 
-fun index_nat :: "nat \<Rightarrow> nat \<Rightarrow> nat" where 
+fun index_nat :: "nat \<Rightarrow> nat \<Rightarrow> nat" where
 "index_nat xs a = (if xs = 0 then 0 else if hd_nat xs = a then 0 else 1 + index_nat (tl_nat xs) a)"
 
 lemma sub_index:
@@ -2059,27 +2070,27 @@ lemma sub_index:
   apply (induct xs)
    apply simp
   apply (subst index_nat.simps)
-  apply (auto simp add: sub_hd list_encode_eq sub_tl inj_def 
+  apply (auto simp add: sub_hd list_encode_eq sub_tl inj_def
           simp del:index_nat.simps simp flip:list_encode.simps)
   done
 
-definition sat_formula_list_encode :: "sat_plan_formula list \<Rightarrow>nat" where 
+definition sat_formula_list_encode :: "sat_plan_formula list \<Rightarrow>nat" where
 "sat_formula_list_encode xs = list_encode (map sat_formula_encode xs)"
 
-definition sat_formula_list_decode :: "nat \<Rightarrow> sat_plan_formula list" where 
+definition sat_formula_list_decode :: "nat \<Rightarrow> sat_plan_formula list" where
 "sat_formula_list_decode n = map sat_formula_decode (list_decode n)"
 
-lemma sat_formula_list_id: 
+lemma sat_formula_list_id:
 "sat_formula_list_decode (sat_formula_list_encode x) = x"
   apply (auto simp add:sat_formula_list_decode_def sat_formula_list_encode_def)
-  using sat_formula_id 
+  using sat_formula_id
   by (simp add: map_idI)
 
-fun BigAnd_nat:: "nat \<Rightarrow> nat" where 
+fun BigAnd_nat:: "nat \<Rightarrow> nat" where
 "BigAnd_nat xs = (if xs=0 then 2##(0##0)##0 else 3##(hd_nat xs)##(BigAnd_nat (tl_nat xs))##0)"
 
-fun BigAnd_acc:: "nat \<Rightarrow> nat \<Rightarrow> nat" where 
-"BigAnd_acc acc xs = (if xs=0 then acc 
+fun BigAnd_acc:: "nat \<Rightarrow> nat \<Rightarrow> nat" where
+"BigAnd_acc acc xs = (if xs=0 then acc
  else BigAnd_acc (3##(hd_nat xs)## acc ##0) (tl_nat xs))"
 
 
@@ -2093,11 +2104,11 @@ lemma sub_BigAnd:
 simp del:BigAnd_nat.simps)
   done
 
-lemma BigAnd_induct : 
+lemma BigAnd_induct :
 " BigAnd_nat (append_nat (reverse_nat xs) ys) = BigAnd_acc (BigAnd_nat ys) xs"
 proof -
   obtain xs' ys' where "xs =list_encode xs' " "ys = list_encode ys'"
-    
+
     by (metis list_decode_inverse)
   thus ?thesis apply (auto simp only: sub_reverse sub_BigAnd sub_append)
     apply(induct xs' arbitrary:ys' xs ys )
@@ -2111,7 +2122,7 @@ proof -
         simp del:BigAnd_nat.simps BigAnd_acc.simps simp flip:list_encode.simps)
     done
 qed
-definition BigAnd_tail :: "nat \<Rightarrow> nat" where 
+definition BigAnd_tail :: "nat \<Rightarrow> nat" where
 "BigAnd_tail xs = BigAnd_acc (2##(0##0)##0) (reverse_nat xs) "
 
 lemma subtail_BigAnd :
@@ -2130,18 +2141,18 @@ lemma sub_BigOr:
 simp del:BigOr_nat.simps)
   done
 
-fun BigOr_acc:: "nat \<Rightarrow> nat \<Rightarrow> nat" where 
-"BigOr_acc acc xs = (if xs=0 then acc 
+fun BigOr_acc:: "nat \<Rightarrow> nat \<Rightarrow> nat" where
+"BigOr_acc acc xs = (if xs=0 then acc
  else BigOr_acc (4##(hd_nat xs)## acc ##0) (tl_nat xs))"
 
 
 
 
-lemma BigOr_induct : 
+lemma BigOr_induct :
 " BigOr_nat (append_nat (reverse_nat xs) ys) = BigOr_acc (BigOr_nat ys) xs"
 proof -
   obtain xs' ys' where "xs =list_encode xs' " "ys = list_encode ys'"
-    
+
     by (metis list_decode_inverse)
   thus ?thesis apply (auto simp only: sub_reverse sub_BigAnd sub_append)
     apply(induct xs' arbitrary:ys' xs ys )
@@ -2155,7 +2166,7 @@ proof -
     done
 qed
 
-definition BigOr_tail :: "nat \<Rightarrow> nat" where 
+definition BigOr_tail :: "nat \<Rightarrow> nat" where
 "BigOr_tail xs = BigOr_acc (0##0) (reverse_nat xs) "
 
 lemma subtail_BigOr :
@@ -2166,10 +2177,10 @@ lemma strips_simp:"strips_assignment_encode = prod_encode o (\<lambda>(s,b). (sa
   apply (auto)
   done
 
-fun map_pair :: "nat \<Rightarrow> nat \<Rightarrow> nat" where 
+fun map_pair :: "nat \<Rightarrow> nat \<Rightarrow> nat" where
 "map_pair x xs = (if xs = 0 then 0 else (prod_encode (x,hd_nat xs)) ## map_pair x (tl_nat xs))"
 
-fun map_pair_acc :: "nat \<Rightarrow> nat \<Rightarrow> nat \<Rightarrow> nat" where 
+fun map_pair_acc :: "nat \<Rightarrow> nat \<Rightarrow> nat \<Rightarrow> nat" where
 "map_pair_acc acc x xs = (if xs = 0 then acc else map_pair_acc ((prod_encode (x,hd_nat xs)) ## acc) x (tl_nat xs))"
 
 lemma submap_pair:
@@ -2177,30 +2188,30 @@ lemma submap_pair:
   apply (induct xs)
    apply simp
   apply (subst map_pair.simps)
-  apply (auto simp add: sub_cons cons0 sub_hd sub_tl 
+  apply (auto simp add: sub_cons cons0 sub_hd sub_tl
 list_encode_eq simp del: map_pair.simps
-simp flip: list_encode.simps 
+simp flip: list_encode.simps
 )
   done
 
-lemma submap_pair_gen: 
+lemma submap_pair_gen:
 "map_pair x (list_encode xs) = list_encode  (map (prod_encode o Pair x) xs) "
   using submap_pair[of id x id xs] apply auto
-  done 
+  done
 
 lemma submap_pair_mappair:
 "map_pair x xs = map_nat (prod_encode o Pair x) xs"
-using submap_pair_gen sub_map 
+using submap_pair_gen sub_map
   by (metis list_decode_inverse)
 
 
 
-fun product_nat :: "nat \<Rightarrow> nat \<Rightarrow> nat" where 
+fun product_nat :: "nat \<Rightarrow> nat \<Rightarrow> nat" where
 "product_nat xs ys = (if xs = 0 then 0 else append_nat (map_pair (hd_nat xs) ys) (product_nat (tl_nat xs) ys))"
 
 
 lemma sub_product:
-"product_nat (list_encode (map f xs)) (list_encode (map g ys)) 
+"product_nat (list_encode (map f xs)) (list_encode (map g ys))
 = list_encode (map (\<lambda>(x,y). prod_encode (f x, g y)) (List.product xs ys))"
   apply (induct xs)
    apply simp
@@ -2211,7 +2222,7 @@ sub_hd head.simps)
   done
 
 lemma sub_product_id:
-"product_nat (list_encode xs) (list_encode ys) 
+"product_nat (list_encode xs) (list_encode ys)
 = list_encode (map prod_encode (List.product xs ys))"
   using sub_product[of id xs id ys] by simp
 
@@ -2219,11 +2230,11 @@ lemma sub_elem_of_inj: "inj f \<Longrightarrow> (elemof (f e) (list_encode (map 
   apply (induct l)
    apply simp
   apply (subst elemof.simps)
-  apply (auto simp add: inj_def 
+  apply (auto simp add: inj_def
       list_encode_eq sub_hd sub_tl simp del:elemof.simps simp flip: list_encode.simps)
   done
 
-fun map_acc :: "(nat \<Rightarrow> nat) \<Rightarrow> nat \<Rightarrow> nat \<Rightarrow> nat" where 
+fun map_acc :: "(nat \<Rightarrow> nat) \<Rightarrow> nat \<Rightarrow> nat \<Rightarrow> nat" where
 "map_acc f acc n = (if n = 0 then acc else map_acc f ((f (hd_nat n)) ## acc) (tl_nat n))"
 
 lemma rev_cons: "a # rev xs = rev (xs @[a])"
@@ -2236,15 +2247,15 @@ lemma append_singleton:
 lemma map_induct :
 "reverse_nat (map_nat f (append_nat xs ys))
 = map_acc f (reverse_nat ( map_nat f xs)) ys"
-proof - 
+proof -
   obtain xs' ys' where "xs = list_encode xs'" "ys = list_encode ys'"
     by (metis list_decode_inverse)
-  thus ?thesis  
-    apply(auto simp only: sub_append sub_map sub_reverse) 
+  thus ?thesis
+    apply(auto simp only: sub_append sub_map sub_reverse)
     apply(induct ys' arbitrary:xs' xs ys)
      apply simp
     apply(subst map_acc.simps)
-    apply(auto simp add: sub_tl sub_hd sub_cons 
+    apply(auto simp add: sub_tl sub_hd sub_cons
             simp del:map_acc.simps list_encode.simps)
      apply simp
     subgoal for a ys' xs'
@@ -2253,13 +2264,13 @@ proof -
     done
 qed
 
-      
+
 lemma subtail_map:
 "reverse_nat (map_acc f  0 xs) = map_nat f xs"
-  using map_induct[of f 0 xs] 
+  using map_induct[of f 0 xs]
   by (metis append_nat.simps(1) map_nat.simps rev_rev_nat reverse_nat_0)
 
-fun filter_acc :: "(nat \<Rightarrow> bool) \<Rightarrow> nat \<Rightarrow> nat \<Rightarrow> nat" where 
+fun filter_acc :: "(nat \<Rightarrow> bool) \<Rightarrow> nat \<Rightarrow> nat \<Rightarrow> nat" where
 "filter_acc f acc xs = (if xs = 0 then acc else if f (hd_nat xs) then filter_acc f ((hd_nat xs) ## acc) (tl_nat xs)
 else filter_acc  f  acc (tl_nat xs))"
 
@@ -2271,11 +2282,11 @@ lemma filter_append:
 lemma filter_induct:
 "reverse_nat (filter_nat f (append_nat xs ys))
 = filter_acc f (reverse_nat ( filter_nat f xs)) ys"
-proof - 
+proof -
   obtain xs' ys' where "xs = list_encode xs'" "ys = list_encode ys'"
     by (metis list_decode_inverse)
-  thus ?thesis  
-    apply(auto simp only: sub_append sub_filter sub_reverse) 
+  thus ?thesis
+    apply(auto simp only: sub_append sub_filter sub_reverse)
     apply(induct ys' arbitrary:xs' xs ys)
      apply simp
     apply(subst filter_acc.simps)
@@ -2289,7 +2300,7 @@ qed
 
 lemma subtail_filter:
 "reverse_nat (filter_acc f  0 xs) = filter_nat f xs"
-  using filter_induct[of f 0 xs] 
+  using filter_induct[of f 0 xs]
   by (metis append_nat.simps(1) filter_nat.simps rev_rev_nat reverse_nat_0)
 
 lemma map_pair_induct :
@@ -2298,15 +2309,15 @@ lemma map_pair_induct :
   apply auto
   done
 
-definition map_pair_tail :: "nat \<Rightarrow> nat \<Rightarrow> nat" where 
+definition map_pair_tail :: "nat \<Rightarrow> nat \<Rightarrow> nat" where
 "map_pair_tail x xs = reverse_nat (map_pair_acc 0 x xs)"
 
 lemma subtail_map_pair:
 "map_pair_tail x xs = map_pair x xs"
   using map_pair_tail_def map_pair_induct submap_pair_mappair subtail_map by presburger
 
-fun product_acc :: "nat \<Rightarrow> nat \<Rightarrow> nat \<Rightarrow> nat" where 
-"product_acc acc xs ys = (if xs = 0 then acc else 
+fun product_acc :: "nat \<Rightarrow> nat \<Rightarrow> nat \<Rightarrow> nat" where
+"product_acc acc xs ys = (if xs = 0 then acc else
 product_acc (append_tail ( reverse_nat (map_pair_tail (hd_nat xs) ys)) acc ) (tl_nat xs) ys)"
 
 
@@ -2321,8 +2332,8 @@ proof -
      apply simp
     apply (subst product_acc.simps)
     apply (auto simp add: non_empty_not_zero subtail_append sub_reverse sub_hd subtail_map_pair
-      submap_pair_mappair sub_map sub_append sub_tl 
- simp flip: map_append 
+      submap_pair_mappair sub_map sub_append sub_tl
+ simp flip: map_append
           simp del: product_acc.simps product_nat.simps list_encode.simps map_pair.simps map_nat.simps)
     apply force
     done
@@ -2332,14 +2343,14 @@ qed
 definition product_tail :: "nat \<Rightarrow> nat \<Rightarrow> nat" where
 "product_tail xs ys = reverse_nat (product_acc 0 xs ys)"
 
-lemma subtail_product: 
+lemma subtail_product:
 "product_tail xs ys = product_nat xs ys "
   using append_nat_0 product_induct product_tail_def rev_rev_nat by presburger
 
-fun map_snd_acc  :: "nat \<Rightarrow> nat \<Rightarrow> nat " where 
+fun map_snd_acc  :: "nat \<Rightarrow> nat \<Rightarrow> nat " where
 "map_snd_acc acc xs = (if xs = 0 then acc else map_snd_acc ((snd_nat (hd_nat xs)) ##acc) (tl_nat xs))"
 
-lemma map_snd_induct: 
+lemma map_snd_induct:
 "map_snd_acc acc xs = map_acc snd_nat acc xs"
   apply(induct acc xs rule:map_snd_acc.induct)
   apply auto
@@ -2361,8 +2372,8 @@ proof -
     done
 qed
 
-fun del_acc :: "nat \<Rightarrow>nat \<Rightarrow> nat \<Rightarrow> nat" where 
-"del_acc acc xs a = (if xs =0 then acc else if fst_nat (hd_nat xs) = a then del_acc acc (tl_nat xs) a else del_acc 
+fun del_acc :: "nat \<Rightarrow>nat \<Rightarrow> nat \<Rightarrow> nat" where
+"del_acc acc xs a = (if xs =0 then acc else if fst_nat (hd_nat xs) = a then del_acc acc (tl_nat xs) a else del_acc
   ((hd_nat xs)##acc)  (tl_nat xs) a )"
 
 lemma del_induct :
@@ -2371,7 +2382,7 @@ lemma del_induct :
   apply auto
   done
 
-definition del_tail :: "nat \<Rightarrow> nat \<Rightarrow> nat" where 
+definition del_tail :: "nat \<Rightarrow> nat \<Rightarrow> nat" where
 "del_tail xs a = reverse_nat (del_acc 0 xs a) "
 
 lemma subtail_del:
@@ -2379,7 +2390,7 @@ lemma subtail_del:
   using del_tail_def del_induct del_filter_nat subtail_filter by presburger
 
 function nub_acc :: "nat \<Rightarrow> nat \<Rightarrow> nat" where
-"nub_acc acc xs = (if xs = 0 then acc else nub_acc ((hd_nat xs) ## acc) 
+"nub_acc acc xs = (if xs = 0 then acc else nub_acc ((hd_nat xs) ## acc)
       (del_tail xs (fst_nat (hd_nat xs))))"
  by pat_completeness auto
 termination
@@ -2401,7 +2412,7 @@ termination
   qed
   done
 
-lemma nub_induct: 
+lemma nub_induct:
 "nub_acc acc xs = append_nat (reverse_nat (nub_nat xs)) acc "
 proof -
   obtain xs' acc' where "xs =list_encode (map prod_encode xs')" "acc =list_encode acc'"
@@ -2413,28 +2424,28 @@ proof -
     apply (auto simp only:subtail_del sub_del sub_hd head.simps list.simps sub_fst fst_conv sub_cons )
     apply(auto simp only: sub_del  simp flip: list.map )
     by (metis (no_types, lifting) append.assoc append.left_neutral
- del.simps(2) list.simps(3) list.simps(9) list_encode.simps(1) list_encode_eq 
-nub.simps(2) rev_append rev_cons rev_rev_ident) 
+ del.simps(2) list.simps(3) list.simps(9) list_encode.simps(1) list_encode_eq
+nub.simps(2) rev_append rev_cons rev_rev_ident)
 qed
 
-definition nub_tail :: "nat \<Rightarrow> nat" where 
+definition nub_tail :: "nat \<Rightarrow> nat" where
 "nub_tail xs = reverse_nat (nub_acc 0 xs)"
 
 lemma subtail_nub:
 "nub_tail xs = nub_nat xs"
   using append_nat_0 nub_induct nub_tail_def rev_rev_nat by presburger
 
-definition ran_tail :: "nat \<Rightarrow> nat" where 
+definition ran_tail :: "nat \<Rightarrow> nat" where
 "ran_tail xs = map_snd_tail (nub_tail xs)"
 
 lemma subtail_ran:
 "ran_tail xs = ran_nat xs"
   using ran_nat_def ran_tail_def subtail_map_snd subtail_nub by presburger
 
-fun length_acc :: "nat \<Rightarrow> nat \<Rightarrow> nat" where 
+fun length_acc :: "nat \<Rightarrow> nat \<Rightarrow> nat" where
 "length_acc acc xs = (if xs = 0 then acc else length_acc (acc+1) (tl_nat xs))"
 
-lemma length_induct: 
+lemma length_induct:
 "length_acc acc xs = length_nat xs + acc"
 proof -
   obtain xs' where "xs = list_encode xs'"
@@ -2446,7 +2457,7 @@ proof -
     apply( auto simp add: non_empty_positive sub_tl simp del:length_acc.simps list_encode.simps(2))
     done
 qed
-definition length_tail :: "nat \<Rightarrow> nat" where 
+definition length_tail :: "nat \<Rightarrow> nat" where
 "length_tail xs = length_acc 0 xs"
 
 lemma subtail_length :
